chore(cleaning project): remove the unused files inherited from Cerise

theories/examples/macros.v
@@ -1,158 +1,103 @@
 From iris.algebra Require Import frac.
-From iris.proofmode Require Import proofmode.
+From iris.proofmode Require Import proofmode spec_patterns coq_tactics ltac_tactics reduction.
 Require Import Eqdep_dec List.
 From cap_machine Require Import rules logrel.
-From cap_machine.proofmode Require Import tactics_helpers map_simpl solve_pure.
 From cap_machine Require Export iris_extra addr_reg_sample contiguous malloc assert.
+(* From cap_machine Require Export salloc. *)
+From cap_machine.proofmode Require Import classes tactics_helpers solve_pure proofmode map_simpl.
 
 Section macros.
-  Context {Σ:gFunctors} {ceriseg:ceriseG Σ}
+  Context {Σ:gFunctors} {ceriseg:ceriseG Σ} {seals:sealStoreG Σ}
           {nainv: logrel_na_invs Σ}
           `{reservedaddresses : ReservedAddresses}
           `{MP: MachineParameters}.
-
 
   (* --------------------------------------------------------------------------------- *)
   (* ------------------------------------- FETCH ------------------------------------- *)
   (* --------------------------------------------------------------------------------- *)
 
-  Definition fetch_instrs (f : Z) :=
+  Definition fetch_instrs (f : Z) : list LWord :=
     encodeInstrsLW [
-        Mov r_t1 PC;
-        GetB r_t2 r_t1;
-        GetA r_t3 r_t1;
-        Sub r_t2 r_t2 r_t3;
-        Lea r_t1 r_t2;
-        Load r_t1 r_t1;
-        Lea r_t1 f;
-        Mov r_t2 0;
-        Mov r_t3 0;
-        Load r_t1 r_t1].
+      Mov r_t1 PC;
+      GetB r_t2 r_t1;
+      GetA r_t3 r_t1;
+      Sub r_t2 r_t2 r_t3;
+      Lea r_t1 r_t2;
+      Load r_t1 r_t1;
+      Lea r_t1 f;
+      Mov r_t2 0;
+      Mov r_t3 0;
+      Load r_t1 r_t1
+    ].
 
-  Definition fetch f a v : iProp Σ :=
-    ([∗ list] a_i;w_i ∈ a;(fetch_instrs f), (a_i, v) ↦ₐ w_i)%I.
-
-  (* fetch spec *)
-  Lemma fetch_spec f a (v : Version) pc_p pc_b pc_e a_first a_last b_link e_link a_link entry_a wentry φ w1 w2 w3:
-    isCorrectPC_range pc_p pc_b pc_e a_first a_last ->
-    contiguous_between a a_first a_last ->
+  Lemma fetch_spec f pc_p pc_b pc_e pc_v a_first b_link e_link a_link v_link entry_a wentry φ w1 w2 w3:
+    ExecPCPerm pc_p →
+    SubBounds pc_b pc_e a_first (a_first ^+ length (fetch_instrs f))%a →
     withinBounds b_link e_link entry_a = true ->
     (a_link + f)%a = Some entry_a ->
 
-      ▷ fetch f a v
-    ∗ ▷ PC ↦ᵣ LCap pc_p pc_b pc_e a_first v
-    ∗ ▷ (pc_b, v) ↦ₐ LCap RO b_link e_link a_link v
-    ∗ ▷ (entry_a, v) ↦ₐ wentry
+      ▷ codefrag a_first pc_v (fetch_instrs f)
+    ∗ ▷ PC ↦ᵣ LCap pc_p pc_b pc_e a_first pc_v
+    ∗ ▷ (pc_b,pc_v) ↦ₐ LCap RO b_link e_link a_link v_link
+    ∗ ▷ (entry_a,v_link) ↦ₐ wentry
     ∗ ▷ r_t1 ↦ᵣ w1
     ∗ ▷ r_t2 ↦ᵣ w2
     ∗ ▷ r_t3 ↦ᵣ w3
     (* if the capability is global, we want to be able to continue *)
     (* if w is not a global capability, we will fail, and must now show that Phi holds at failV *)
-    ∗ ▷ (PC ↦ᵣ LCap pc_p pc_b pc_e a_last v
-         ∗ fetch f a v
+    ∗ ▷ (PC ↦ᵣ LCap pc_p pc_b pc_e (a_first ^+ length (fetch_instrs f))%a pc_v
+         ∗ codefrag a_first pc_v (fetch_instrs f)
          (* the newly allocated region *)
          ∗ r_t1 ↦ᵣ wentry ∗ r_t2 ↦ᵣ LInt 0%Z ∗ r_t3 ↦ᵣ LInt 0%Z
-         ∗ (pc_b, v) ↦ₐ LCap RO b_link e_link a_link v
-         ∗ (entry_a, v) ↦ₐ wentry
-           -∗ WP Seq (Instr Executable) {{ φ }})
+         ∗ (pc_b,pc_v) ↦ₐ LCap RO b_link e_link a_link v_link
+         ∗ (entry_a,v_link) ↦ₐ wentry
+         -∗ WP Seq (Instr Executable) {{ φ }})
     ⊢
       WP Seq (Instr Executable) {{ φ }}.
   Proof.
     iIntros (Hvpc Hcont Hwb Hentry) "(>Hprog & >HPC & >Hpc_b & >Ha_entry & >Hr_t1 & >Hr_t2 & >Hr_t3 & Hφ)".
-    iDestruct (big_sepL2_length with "Hprog") as %Hlength.
-    destruct a as [|a l];[inversion Hlength|].
-    apply contiguous_between_cons_inv_first in Hcont as Heq. subst.
-    (* move r_t1 PC *)
-    destruct l;[inversion Hlength|].
-    iPrologue "Hprog".
-    iApply (wp_move_success_reg_fromPC with "[$HPC $Hi $Hr_t1]");
-      [apply decode_encode_instrW_inv|iCorrectLPC a_first a_last|iContiguous_next Hcont 0|auto|..].
-    iEpilogue "(HPC & Hprog_done & Hr_t1)".
-    (* getb r_t2 r_t1 *)
-    destruct l;[inversion Hlength|].
-    iPrologue "Hprog".
-    iApply (wp_Get_success with "[$HPC $Hi $Hr_t1 $Hr_t2 ]");
-      [apply decode_encode_instrW_inv|auto|iCorrectLPC a_first a_last|iContiguous_next Hcont 1|auto..].
-    iEpilogue "(HPC & Hi & Hr_t1 & Hr_t2) /="; iCombine "Hi" "Hprog_done" as "Hprog_done".
-    (* geta r_t3 r_t1 *)
-    destruct l;[inversion Hlength|].
-    iPrologue "Hprog".
-    iApply (wp_Get_success with "[$HPC $Hi $Hr_t1 $Hr_t3]");
-      [apply decode_encode_instrW_inv|auto|iCorrectLPC a_first a_last|iContiguous_next Hcont 2|auto..].
-    iEpilogue "(HPC & Hi & Hr_t1 & Hr_t3) /="; iCombine "Hi" "Hprog_done" as "Hprog_done".
-    (* sub r_t2 r_t2 r_t3 *)
-    destruct l;[inversion Hlength|].
-    iPrologue "Hprog".
-    iApply (wp_add_sub_lt_success_dst_r with "[$HPC $Hi $Hr_t3 $Hr_t2]");
-      [apply decode_encode_instrW_inv|auto|iContiguous_next Hcont 3|iCorrectLPC a_first a_last|..].
-    iEpilogue "(HPC & Hi & Hr_t3 & Hr_t2) /="; iCombine "Hi" "Hprog_done" as "Hprog_done".
-    (* lea r_t1 r_t2 *)
-    destruct l;[inversion Hlength|].
-    iPrologue "Hprog".
-    assert ((a_first + (pc_b - a_first))%a = Some pc_b) as Hlea;[solve_addr|].
-    iApply (wp_lea_success_reg with "[$HPC $Hi $Hr_t1 $Hr_t2]");
-      [apply decode_encode_instrW_inv|iCorrectLPC a_first a_last|iContiguous_next Hcont 4|apply Hlea|auto..].
-    { apply contiguous_between_length in Hcont.
-      apply isCorrectPC_range_perm in Hvpc; [|revert Hcont; clear; solve_addr].
-      destruct Hvpc as [-> | ->]; auto. }
-    iEpilogue "(HPC & Hi & Hr_t2 & Hr_t1) /="; iCombine "Hi" "Hprog_done" as "Hprog_done".
-    (* load r_t1 r_t1 *)
-    destruct l;[inversion Hlength|].
-    iPrologue "Hprog".
-    iAssert (⌜(pc_b ≠ f4)%Z⌝)%I as %Hneq.
-    { iIntros (Hcontr);subst. iApply (addr_dupl_false with "Hi Hpc_b"). }
-    iApply (wp_load_success_same with "[$HPC $Hi $Hr_t1 Hpc_b]");
-      [|apply decode_encode_instrW_inv|iCorrectLPC a_first a_last| | |iContiguous_next Hcont 5|..].
-    { exact (LCap RW b_link e_link a_link v). }
-    { apply contiguous_between_length in Hcont as Hlen.
-      assert (pc_b < pc_e)%Z as Hle.
-      { eapply isCorrectPC_contiguous_range in Hvpc as Hwb';[|eauto|apply elem_of_cons;left;eauto].
-        inversion Hwb'. solve_addr. }
-      apply isCorrectPC_range_perm in Hvpc as Heq; [|revert Hlen; clear; solve_addr].
-      destruct Heq as [-> | ->]; auto. }
-    { apply andb_true_intro. split;[apply Z.leb_le;solve_addr|apply Z.ltb_lt;auto].
-      assert (pc_b < pc_e)%Z as Hle.
-      { eapply isCorrectPC_contiguous_range in Hvpc as Hwb';[|eauto|apply elem_of_cons;left;eauto].
-        inversion Hwb'. solve_addr. } auto. }
-    { destruct (pc_b =? f4)%a ; [by rewrite Nat.eqb_refl andb_true_l|iFrame].
-    }
-    destruct ((pc_b =? f4)%a) eqn:Hcontr;[apply Z.eqb_eq in Hcontr;apply finz_to_z_eq in Hcontr;congruence|clear Hcontr].
-    iEpilogue "(HPC & Hr_t1 & Hi & Hpc_b)"; iCombine "Hi" "Hprog_done" as "Hprog_done".
-    (* lea r_t1 f *)
-    destruct l;[inversion Hlength|].
-    iPrologue "Hprog".
-    iApply (wp_lea_success_z with "[$HPC $Hi $Hr_t1]");
-      [apply decode_encode_instrW_inv|iCorrectLPC a_first a_last|iContiguous_next Hcont 6|apply Hentry|simpl;auto..].
-    iEpilogue "(HPC & Hi & Hr_t1)"; iCombine "Hi" "Hprog_done" as "Hprog_done".
-    (* move r_t2 0 *)
-    destruct l;[inversion Hlength|].
-    iPrologue "Hprog".
-    iApply (wp_move_success_z with "[$HPC $Hi $Hr_t2]");
-      [apply decode_encode_instrW_inv|iCorrectLPC a_first a_last|iContiguous_next Hcont 7|auto|..].
-    iEpilogue "(HPC & Hi & Hr_t2)"; iCombine "Hi" "Hprog_done" as "Hprog_done".
-    (* move r_t3 0 *)
-    destruct l;[inversion Hlength|].
-    iPrologue "Hprog".
-    iApply (wp_move_success_z with "[$HPC $Hi $Hr_t3]");
-      [apply decode_encode_instrW_inv|iCorrectLPC a_first a_last|iContiguous_next Hcont 8|auto|..].
-    iEpilogue "(HPC & Hi & Hr_t3)"; iCombine "Hi" "Hprog_done" as "Hprog_done".
-    (* load r_t1 r_t1 *)
-    destruct l;[|inversion Hlength].
-    apply contiguous_between_last with (ai:=f8) in Hcont as Hlink;[|auto].
-    iPrologue "Hprog".
-    iAssert (⌜(entry_a ≠ f8)%Z⌝)%I as %Hneq'.
-    { iIntros (Hcontr);subst. iApply (addr_dupl_false with "Hi Ha_entry"). }
-    iApply (wp_load_success_same with "[$HPC $Hi $Hr_t1 Ha_entry]");
-      [exact wentry|apply decode_encode_instrW_inv|iCorrectLPC a_first a_last|auto|auto|apply Hlink|..].
-    { destruct (entry_a =? f8)%a; auto ; by rewrite Nat.eqb_refl andb_true_l. }
-    destruct ((entry_a =? f8)%a) eqn:Hcontr;[apply Z.eqb_eq in Hcontr;apply finz_to_z_eq in Hcontr;congruence|clear Hcontr].
-    iEpilogue "(HPC & Hr_t1 & Hi & Hentry_a)"; iCombine "Hi" "Hprog_done" as "Hprog_done".
-    (* continuation *)
-    iApply "Hφ".
-    iFrame.
-    do 9 iDestruct "Hprog_done" as "[$ Hprog_done]".
-    iFrame.
-  Qed.
+    codefrag_facts "Hprog".
+    iGo "Hprog". transitivity (Some pc_b); eauto. solve_addr.
+    iGo "Hprog". iApply "Hφ"; iFrame.
+ Qed.
+
+  (* --------------------------------------------------------------------------------- *)
+  (* ----------------------------------- FETCH BIS ----------------------------------- *)
+  (* --------------------------------------------------------------------------------- *)
+
+  Definition fetch_reg_instrs (f : Z) (r_lt : RegName): list LWord :=
+    (* r_lt := (RO, b_lt, e_lt, b_tbl) ; linking table capability *)
+    encodeInstrsLW [
+        Lea r_lt f; (* r_lt := (RO, b_lt, e_lt, b_tbl + f) *)
+        Load r_lt r_lt (* r_lt := mem(b_tbl + f) *)
+      ].
+
+  Lemma fetch_reg_spec f r_lt pc_p pc_b pc_e pc_v a_first b_link e_link a_link v_link entry_a wentry φ :
+    ExecPCPerm pc_p →
+    SubBounds pc_b pc_e a_first (a_first ^+ length (fetch_reg_instrs f r_lt))%a →
+    withinBounds b_link e_link entry_a = true ->
+    (a_link + f)%a = Some entry_a ->
+
+      ▷ codefrag a_first pc_v (fetch_reg_instrs f r_lt)
+    ∗ ▷ PC ↦ᵣ LCap pc_p pc_b pc_e a_first pc_v
+    ∗ ▷ (entry_a,v_link) ↦ₐ wentry
+    ∗ ▷ r_lt ↦ᵣ LCap RO b_link e_link a_link v_link
+    (* if the capability is global, we want to be able to continue *)
+    (* if w is not a global capability, we will fail, and must now show that Phi holds at failV *)
+    ∗ ▷ (PC ↦ᵣ LCap pc_p pc_b pc_e (a_first ^+ length (fetch_reg_instrs f r_lt))%a pc_v
+         ∗ codefrag a_first pc_v (fetch_reg_instrs f r_lt)
+         (* the newly allocated region *)
+         ∗ r_lt ↦ᵣ wentry
+         ∗ (entry_a,v_link) ↦ₐ wentry
+         -∗ WP Seq (Instr Executable) {{ φ }})
+    ⊢
+      WP Seq (Instr Executable) {{ φ }}.
+  Proof.
+    iIntros (Hvpc Hcont Hwb Hentry) "(>Hprog & >HPC & >Ha_entry & >Hr_t1 & Hφ)".
+    codefrag_facts "Hprog".
+    iGo "Hprog".
+    iApply "Hφ"; iFrame.
+ Qed.
 
   (* --------------------------------------------------------------------------------- *)
   (* ------------------------------------- ASSERT ------------------------------------ *)
@@ -160,133 +105,139 @@ Section macros.
 
   Definition assert_instrs f_a :=
     fetch_instrs f_a ++
-      encodeInstrsLW [
-        Mov r_t2 r_t0;
-        Mov r_t0 PC;
-        Lea r_t0 3;
-        Jmp r_t1;
-        Mov r_t0 r_t2;
-        Mov r_t1 0;
-        Mov r_t2 0].
-
-  Definition assert a f_a v :=
-    ([∗ list] a_i;w_i ∈ a;(assert_instrs f_a), (a_i, v) ↦ₐ w_i)%I.
+    encodeInstrsLW [
+      Mov r_t2 r_t0;
+      Mov r_t0 PC;
+      Lea r_t0 3;
+      Jmp r_t1;
+      Mov r_t0 r_t2;
+      Mov r_t1 0;
+      Mov r_t2 0
+    ].
 
   (* Spec for assertion success *)
-  (* Since we are not jumping to the failure subroutine, we do not need any assumptions
-     about the failure subroutine *)
-  Lemma assert_success a f_a pc_p pc_b pc_e v a_first a_last
-        b_link e_link a_link a_entry w0 w1 w2 w3 n1 n2
-        ba a_flag ea assertN EN φ :
-    isCorrectPC_range pc_p pc_b pc_e a_first a_last →
-    contiguous_between a a_first a_last →
+  Lemma assert_success f_a pc_p pc_b pc_e pc_v a_first
+        b_link e_link a_link v_link a_entry ba a_flag ea v_assert w0 w1 w2 w3 assertN EN n1 n2 φ :
+    ExecPCPerm pc_p →
+    SubBounds pc_b pc_e a_first (a_first ^+ length (assert_instrs f_a))%a →
     (* linking table assumptions *)
     withinBounds b_link e_link a_entry = true →
-    (a_link + f_a)%a = Some a_entry →
+    (a_link + f_a)%a = Some a_entry ->
     ↑assertN ⊆ EN →
     (* condition for assertion success *)
     (n1 = n2) →
 
-    ▷ assert a f_a v
-    ∗ na_inv logrel_nais assertN (assert_inv ba a_flag ea v)
+    ▷ codefrag a_first pc_v (assert_instrs f_a)
+    ∗ na_inv logrel_nais assertN (assert_inv ba a_flag ea v_assert)
     ∗ na_own logrel_nais EN
-    ∗ ▷ PC ↦ᵣ LCap pc_p pc_b pc_e a_first v
-    ∗ ▷ (pc_b, v) ↦ₐ LCap RO b_link e_link a_link v
-    ∗ ▷ (a_entry, v) ↦ₐ LCap E ba ea ba v
+    ∗ ▷ PC ↦ᵣ LCap pc_p pc_b pc_e a_first pc_v
+    ∗ ▷ (pc_b,pc_v) ↦ₐ LCap RO b_link e_link a_link v_link
+    ∗ ▷ (a_entry,v_link) ↦ₐ LCap E ba ea ba v_assert
     ∗ ▷ r_t0 ↦ᵣ w0
     ∗ ▷ r_t1 ↦ᵣ w1
     ∗ ▷ r_t2 ↦ᵣ w2
     ∗ ▷ r_t3 ↦ᵣ w3
     ∗ ▷ r_t4 ↦ᵣ LInt n1
     ∗ ▷ r_t5 ↦ᵣ LInt n2
-    ∗ ▷ (r_t0 ↦ᵣ w0 ∗
-         r_t1 ↦ᵣ LInt 0%Z ∗ r_t2 ↦ᵣ LInt 0%Z ∗ r_t3 ↦ᵣ LInt 0%Z
+    ∗ ▷ (PC ↦ᵣ LCap pc_p pc_b pc_e (a_first ^+ length (assert_instrs f_a))%a pc_v
+         ∗ r_t0 ↦ᵣ w0
+         ∗ r_t1 ↦ᵣ LInt 0%Z ∗ r_t2 ↦ᵣ LInt 0%Z ∗ r_t3 ↦ᵣ LInt 0%Z
          ∗ r_t4 ↦ᵣ LInt 0%Z ∗ r_t5 ↦ᵣ LInt 0%Z
-         ∗ PC ↦ᵣ LCap pc_p pc_b pc_e a_last v
-         ∗ assert a f_a v
+         ∗ codefrag a_first pc_v (assert_instrs f_a)
          ∗ na_own logrel_nais EN
-         ∗ (pc_b,v) ↦ₐ LCap RO b_link e_link a_link v
-         ∗ (a_entry,v) ↦ₐ LCap E ba ea ba v
+         ∗ (pc_b,pc_v) ↦ₐ LCap RO b_link e_link a_link v_link
+         ∗ (a_entry,v_link) ↦ₐ LCap E ba ea ba v_assert
          -∗ WP Seq (Instr Executable) {{ φ }})
     ⊢
     WP Seq (Instr Executable) {{ φ }}.
   Proof.
     iIntros (Hvpc Hcont Hwb Htable HN Hsuccess)
-            "(>Hprog & #Hinv & Hna & >HPC & >Hpc_b & >Ha_entry & >Hr_t0 & >Hr_t1 & >Hr_t2 & >Hr_t3 & >Hr_t4 & >Hr_t5 & Hφ)".
-    iDestruct ( (contiguous_betweenL_program_split _ _ (fun la w_i => la ↦ₐ w_i )%I) with "Hprog")
-      as (fetch_prog rest link) "(Hfetch & Hprog & #Hcont)";[apply Hcont|].
-    iDestruct "Hcont" as %(Hcont_fetch & Hcont_rest & Heqapp & Hlink).
-    iApply (fetch_spec with "[- $HPC $Hfetch $Hr_t1 $Hr_t2 $Hr_t3 $Ha_entry $Hpc_b]");
-      [|apply Hcont_fetch|apply Hwb|apply Htable|].
-    { intros mid Hmid. apply isCorrectPC_inrange with a_first a_last; auto.
-      apply contiguous_between_bounds in Hcont_rest. revert Hcont_rest Hmid; clear. solve_addr. }
-    iNext. iIntros "(HPC & Hfetch& Hr_t1 & Hr_t2 & Hr_t3 & Hpc_b & Ha_entry)".
-    iDestruct (big_sepL2_length with "Hprog") as %Hlength_rest.
-    assert (isCorrectPC_range pc_p pc_b pc_e link a_last) as Hvpc_rest.
-    { intros mid Hmid. apply isCorrectPC_inrange with a_first a_last; auto. revert Hmid Hlink;clear. solve_addr. }
-    destruct rest as [|a0 l'];[inversion Hlength_rest|].
-    apply contiguous_between_cons_inv_first in Hcont_rest as Heq. subst a0.
-    (* move r_t2 r_t0 *)
-    destruct l';[inversion Hlength_rest|]. subst n2.
-    iPrologue "Hprog".
-    iApply (wp_move_success_reg with "[$HPC $Hi $Hr_t2 $Hr_t0]");
-      [apply decode_encode_instrW_inv|iCorrectLPC link a_last|iContiguous_next Hcont_rest 0|].
-    iEpilogue "(HPC & Hi & Hr_t2 & Hr_t0)"; iCombine "Hfetch" "Hi" as "Hprog_done".
-    (* move r_t0 PC *)
-    destruct l';[inversion Hlength_rest|].
-    iPrologue "Hprog".
-    iApply (wp_move_success_reg_fromPC with "[$HPC $Hi $Hr_t0]");
-      [apply decode_encode_instrW_inv|iCorrectLPC link a_last|iContiguous_next Hcont_rest 1|].
-    iEpilogue "(HPC & Hi & Hr_t0)"; iCombine "Hi" "Hprog_done" as "Hprog_done".
-    (* lea r_t0 3 *)
-    destruct l';[inversion Hlength_rest|].
-    destruct l';[inversion Hlength_rest|].
-    iPrologue "Hprog".
-    assert (pc_p ≠ E).
-    { assert (isCorrectLPC (LCap pc_p pc_b pc_e a_first v)) as HH.
-      { apply isCorrectLPC_isCorrectPC_iff.
-        apply Hvpc. split. solve_addr.
-        apply contiguous_between_length in Hcont.
-        rewrite Heqapp app_length /= in Hcont. solve_addr. }
-      destruct pc_p; inversion HH; inversion H0; cbn in *; simplify_eq; destruct_or?; auto.
-    }
-    iApply (wp_lea_success_z with "[$HPC $Hi $Hr_t0]");
-      [apply decode_encode_instrW_inv|iCorrectLPC link a_last|..].
-    { iContiguous_next Hcont_rest 2. }
-    { eapply (contiguous_between_incr_addr_middle' _ _ _ 1%nat 3).
-      apply Hcont_rest. 2: done. 2: done. cbn. lia. } auto.
-    iEpilogue "(HPC & Hi & Hr_t0)"; iCombine "Hi" "Hprog_done" as "Hprog_done".
-    (* jmp r_t1 *)
-    iPrologue "Hprog".
-    iApply (wp_jmp_success with "[$HPC $Hi $Hr_t1]");
-      [apply decode_encode_instrW_inv|iCorrectLPC link a_last|].
-    iEpilogue "(HPC & Hi & Hr_t1)"; iCombine "Hi" "Hprog_done" as "Hprog_done".
-    (* assert routine *)
-    iApply (assert_success_spec with "[- $Hinv $Hna $HPC $Hr_t0 $Hr_t4 $Hr_t5]"); auto.
-    iNext. iIntros "(Hna & HPC & Hr_t0 & Hr_t4 & Hr_t5)".
-    rewrite updatePcPermL_cap_non_E//.
-    (* move r_t0 r_t2 *)
-    destruct l';[inversion Hlength_rest|].
-    iPrologue "Hprog".
-    iApply (wp_move_success_reg with "[$HPC $Hi $Hr_t0 $Hr_t2]");
-      [apply decode_encode_instrW_inv|iCorrectLPC link a_last|iContiguous_next Hcont_rest 4|].
-    iEpilogue "(HPC & Hi & Hr_t0 & Hr_t2)"; iCombine "Hi" "Hprog_done" as "Hprog_done".
-    (* move r_t1 0 *)
-    destruct l';[inversion Hlength_rest|].
-    iPrologue "Hprog".
-    iApply (wp_move_success_z with "[$HPC $Hi $Hr_t1]");
-      [apply decode_encode_instrW_inv|iCorrectLPC link a_last|iContiguous_next Hcont_rest 5|].
-    iEpilogue "(HPC & Hi & Hr_t1)"; iCombine "Hi" "Hprog_done" as "Hprog_done".
-    (* move r_t2 0 *)
-    destruct l';[|inversion Hlength_rest].
-    apply contiguous_between_last with (ai:=f4) in Hcont_rest as Hlink';[|auto].
-    iPrologue "Hprog".
-    iApply (wp_move_success_z with "[$HPC $Hi $Hr_t2]");
-      [apply decode_encode_instrW_inv|iCorrectLPC link a_last|apply Hlink'|auto|..].
-    iEpilogue "(HPC & Hi & Hr_t2)"; iCombine "Hi" "Hprog_done" as "Hprog_done".
-    (* Continuation *)
+            "(>Hprog & #Hinv & Hna & >HPC & >Hpc_b & >Ha_entry & >Hr0 & >Hr1 & >Hr2 & >Hr3
+              & >Hr4 & >Hr5 & Hφ)".
+    rewrite {1}/assert_instrs.
+    focus_block_0 "Hprog" as "Hfetch" "Hcont".
+    iApply fetch_spec; iFrameAutoSolve.
+    iNext. iIntros "(HPC & Hfetch & Hr1 & Hr2 & Hr3 & Hpc_b & Ha_entry)".
+    unfocus_block "Hfetch" "Hcont" as "Hprog".
+
+    focus_block 1 "Hprog" as a_middle Ha_middle "Hprog" "Hcont".
+    do 4 iInstr "Hprog".
+    iApply (assert_success_spec with "[- $Hinv $Hna $HPC $Hr0 $Hr4 $Hr5]"); auto.
+    iNext. iIntros "(Hna & HPC & Hr0 & Hr4 & Hr5)".
+    rewrite updatePcPermL_cap_non_E; [| solve_pure ].
+    iGo "Hprog".
+    unfocus_block "Hprog" "Hcont" as "Hprog".
     iApply "Hφ". iFrame.
-    rewrite Heqapp /=. iDestruct "Hprog_done" as "(?&?&?&?&?&?&?&?)". iFrame. done.
+    changePCto (a_first ^+ length (assert_instrs f_a))%a. iFrame.
+  Qed.
+
+  (* --------------------------------------------------------------------------------- *)
+  (* ----------------------------------- ASSERT BIS ---------------------------------- *)
+  (* --------------------------------------------------------------------------------- *)
+
+  Definition assert_reg_instrs f_a r_lt :=
+    fetch_reg_instrs f_a r_lt ++
+    encodeInstrsLW [
+      Mov r_t2 r_t0;
+      Mov r_t0 PC;
+      Lea r_t0 3;
+      Jmp r_lt;
+      Mov r_t0 r_t2;
+      Mov r_lt 0;
+      Mov r_t2 0
+    ].
+
+  (* Spec for assertion success *)
+  Lemma assert_reg_success f_a r_lt pc_p pc_b pc_e pc_v a_first
+        b_link e_link a_link v_link a_entry ba a_flag ea v_assert w0 w2 assertN EN n1 n2 φ :
+    ExecPCPerm pc_p →
+    SubBounds pc_b pc_e a_first (a_first ^+ length (assert_reg_instrs f_a r_lt))%a →
+    (* linking table assumptions *)
+    withinBounds b_link e_link a_entry = true →
+    (a_link + f_a)%a = Some a_entry ->
+    ↑assertN ⊆ EN →
+    (* condition for assertion success *)
+    (n1 = n2) →
+
+    ▷ codefrag a_first pc_v (assert_reg_instrs f_a r_lt)
+    ∗ na_inv logrel_nais assertN (assert_inv ba a_flag ea v_assert)
+    ∗ na_own logrel_nais EN
+    ∗ ▷ PC ↦ᵣ LCap pc_p pc_b pc_e a_first pc_v
+    ∗ ▷ (a_entry,v_link) ↦ₐ LCap E ba ea ba v_assert
+    ∗ ▷ r_t0 ↦ᵣ w0
+    ∗ ▷ r_lt ↦ᵣ (LCap RO b_link e_link a_link v_link)
+    ∗ ▷ r_t2 ↦ᵣ w2
+    ∗ ▷ r_t4 ↦ᵣ LInt n1
+    ∗ ▷ r_t5 ↦ᵣ LInt n2
+    ∗ ▷ (PC ↦ᵣ LCap pc_p pc_b pc_e (a_first ^+ length (assert_reg_instrs f_a r_lt))%a pc_v
+         ∗ r_t0 ↦ᵣ w0
+         ∗ r_lt ↦ᵣ LInt 0%Z ∗ r_t2 ↦ᵣ LInt 0%Z
+         ∗ r_t4 ↦ᵣ LInt 0%Z ∗ r_t5 ↦ᵣ LInt 0%Z
+         ∗ codefrag a_first pc_v (assert_reg_instrs f_a r_lt)
+         ∗ na_own logrel_nais EN
+         ∗ (a_entry,v_link) ↦ₐ LCap E ba ea ba v_assert
+         -∗ WP Seq (Instr Executable) {{ φ }})
+    ⊢
+    WP Seq (Instr Executable) {{ φ }}.
+  Proof.
+    iIntros (Hvpc Hcont Hwb Htable HN Hsuccess)
+            "(>Hprog & #Hinv & Hna & >HPC & >Ha_entry & >Hr0 & >Hrlt & >Hr2
+              & >Hr4 & >Hr5 & Hφ)".
+    rewrite {1}/assert_reg_instrs.
+    focus_block_0 "Hprog" as "Hfetch" "Hcont".
+    iApply fetch_reg_spec; iFrameAutoSolve.
+    iNext. iIntros "(HPC & Hfetch & Hrlt & Hpc_b & Ha_entry)".
+    unfocus_block "Hfetch" "Hcont" as "Hprog".
+
+    focus_block 1 "Hprog" as a_middle Ha_middle "Hprog" "Hcont".
+    do 4 iInstr "Hprog".
+    iApply (assert_success_spec with "[- $Hinv $Hna $HPC $Hr0 $Hr4 $Hr5]"); auto.
+    iNext. iIntros "(Hna & HPC & Hr0 & Hr4 & Hr5)".
+    rewrite updatePcPermL_cap_non_E; [| solve_pure ].
+    iGo "Hprog".
+    unfocus_block "Hprog" "Hcont" as "Hprog".
+    iApply "Hφ". iFrame.
+    changePCto (a_first ^+ length (assert_reg_instrs f_a r_lt))%a. iFrame.
   Qed.
 
   (* --------------------------------------------------------------------------------- *)
@@ -295,221 +246,53 @@ Section macros.
 
   (* malloc stores the result in r_t1, rather than a user chosen destination.
      f_m is the offset of the malloc capability *)
-  Definition malloc_instrs f_m size :=
+  Definition malloc_instrs f_m (size: Z) :=
     fetch_instrs f_m ++
     encodeInstrsLW [
-    Mov r_t5 r_t0;
-    Mov r_t3 r_t1;
-    Mov r_t1 size;
-    Mov r_t0 PC;
-    Lea r_t0 3;
-    Jmp r_t3;
-    Mov r_t0 r_t5;
-    Mov r_t5 0].
-
-  Definition malloc f_m size a v : iProp Σ :=
-    ([∗ list] a_i;w_i ∈ a;(malloc_instrs f_m size), (a_i,v) ↦ₐ w_i)%I.
+     Mov r_t5 r_t0;
+     Mov r_t3 r_t1;
+     Mov r_t1 size;
+     Mov r_t0 PC;
+     Lea r_t0 3;
+     Jmp r_t3;
+     Mov r_t0 r_t5;
+     Mov r_t5 0
+  ].
 
   (* malloc spec *)
-  Lemma malloc_spec φ size cont a pc_p pc_b pc_e v a_first a_last
-        b_link e_link a_link f_m a_entry mallocN b_m e_m EN rmap :
-    isCorrectPC_range pc_p pc_b pc_e a_first a_last →
-    contiguous_between a a_first a_last →
+  Lemma malloc_spec_alt φ ψ size cont pc_p pc_b pc_e pc_v a_first
+        b_link e_link a_link v_link f_m a_entry v_malloc mallocN b_m e_m EN rmap :
+    ExecPCPerm pc_p →
+    SubBounds pc_b pc_e a_first (a_first ^+ length (malloc_instrs f_m size))%a →
     withinBounds b_link e_link a_entry = true →
     (a_link + f_m)%a = Some a_entry →
     dom rmap = all_registers_s ∖ {[ PC; r_t0 ]} →
     ↑mallocN ⊆ EN →
-    size > 0 →
+    (size > 0)%Z →
 
     (* malloc program and subroutine *)
-    ▷ malloc f_m size a v
-    ∗ na_inv logrel_nais mallocN (malloc_inv b_m e_m v)
+    ▷ codefrag a_first pc_v (malloc_instrs f_m size)
+    ∗ na_inv logrel_nais mallocN (malloc_inv b_m e_m v_malloc)
     ∗ na_own logrel_nais EN
     (* we need to assume that the malloc capability is in the linking table at offset f_m *)
-    ∗ ▷ (pc_b,v) ↦ₐ LCap RO b_link e_link a_link v
-    ∗ ▷ (a_entry,v) ↦ₐ LCap E b_m e_m b_m v
+    ∗ ▷ (pc_b,pc_v) ↦ₐ LCap RO b_link e_link a_link v_link
+    ∗ ▷ (a_entry,v_link) ↦ₐ LCap E b_m e_m b_m v_malloc
     (* register state *)
-    ∗ ▷ PC ↦ᵣ LCap pc_p pc_b pc_e a_first v
-    ∗ ▷ r_t0 ↦ᵣ cont
-    ∗ ▷ ([∗ map] r_i↦w_i ∈ rmap, r_i ↦ᵣ w_i)
-    (* continuation *)
-    ∗ ▷ (PC ↦ᵣ LCap pc_p pc_b pc_e a_last v ∗ malloc f_m size a v
-         ∗ (pc_b,v) ↦ₐ LCap RO b_link e_link a_link v
-         ∗ (a_entry,v) ↦ₐ LCap E b_m e_m b_m v
-         (* the newly allocated region *)
-         ∗ (∃ (b e : Addr),
-            ⌜(b + size)%a = Some e⌝
-            ∗ r_t1 ↦ᵣ LCap RWX b e b v
-            ∗ [[b,e]] ↦ₐ{v} [[region_addrs_zeroesL b e v]])
-         ∗ r_t0 ↦ᵣ cont
-         ∗ na_own logrel_nais EN
-         ∗ ([∗ map] r_i↦w_i ∈ (<[r_t2:=LInt 0%Z]>
-                               (<[r_t3:=LInt 0%Z]>
-                                (<[r_t4:=LInt 0%Z]>
-                                 (<[r_t5:=LInt 0%Z]> (delete r_t1 rmap))))), r_i ↦ᵣ w_i)
-         (* the newly allocated region is fresh in the current world *)
-         (* ∗ ⌜Forall (λ a, a ∉ dom (gset Addr) (std W)) (finz.seq_between b e)⌝ *)
-         -∗ WP Seq (Instr Executable) {{ φ }})
-    ⊢
-      WP Seq (Instr Executable) {{ λ v, φ v ∨ ⌜v = FailedV⌝ }}.
-  Proof.
-    iIntros (Hvpc Hcont Hwb Ha_entry Hrmap_dom HmallocN Hsize)
-            "(>Hprog & #Hmalloc & Hna & >Hpc_b & >Ha_entry & >HPC & >Hr_t0 & >Hregs & Hφ)".
-    (* extract necessary registers from regs *)
-    iDestruct (big_sepL2_length with "Hprog") as %Hlength.
-    assert (is_Some (rmap !! r_t1)) as [rv1 ?]. by rewrite -elem_of_dom Hrmap_dom; set_solver.
-    iDestruct (big_sepM_delete _ _ r_t1 with "Hregs") as "[Hr_t1 Hregs]"; eauto.
-    assert (is_Some (rmap !! r_t2)) as [rv2 ?]. by rewrite -elem_of_dom Hrmap_dom; set_solver.
-    iDestruct (big_sepM_delete _ _ r_t2 with "Hregs") as "[Hr_t2 Hregs]". by rewrite lookup_delete_ne //.
-    assert (is_Some (rmap !! r_t3)) as [rv3 ?]. by rewrite -elem_of_dom Hrmap_dom; set_solver.
-    iDestruct (big_sepM_delete _ _ r_t3 with "Hregs") as "[Hr_t3 Hregs]". by rewrite !lookup_delete_ne //.
-    assert (is_Some (rmap !! r_t5)) as [rv5 ?]. by rewrite -elem_of_dom Hrmap_dom; set_solver.
-    iDestruct (big_sepM_delete _ _ r_t5 with "Hregs") as "[Hr_t5 Hregs]". by rewrite !lookup_delete_ne //.
-    destruct a as [|a l];[inversion Hlength|].
-    apply contiguous_between_cons_inv_first in Hcont as Heq. subst.
-    (* fetch f *)
-    iDestruct ( (contiguous_betweenL_program_split _ _ (fun la w_i => la ↦ₐ w_i )%I) with "Hprog")
-      as (fetch_prog rest link) "(Hfetch & Hprog & #Hcont)";[apply Hcont|].
-    iDestruct "Hcont" as %(Hcont_fetch & Hcont_rest & Heqapp & Hlink).
-    iApply (fetch_spec with "[- $HPC $Hfetch $Hr_t1 $Hr_t2 $Hr_t3 $Ha_entry $Hpc_b]");
-      [|apply Hcont_fetch|apply Hwb|apply Ha_entry|].
-    { intros mid Hmid. apply isCorrectPC_inrange with a_first a_last; auto.
-      apply contiguous_between_bounds in Hcont_rest. revert Hcont_rest Hmid; clear. solve_addr. }
-    iNext. iIntros "(HPC & Hfetch& Hr_t1 & Hr_t2 & Hr_t3 & Hpc_b & Ha_entry)".
-    iDestruct (big_sepL2_length with "Hprog") as %Hlength_rest.
-    assert (isCorrectPC_range pc_p pc_b pc_e link a_last) as Hvpc_rest.
-    { intros mid Hmid. apply isCorrectPC_inrange with a_first a_last; auto. revert Hmid Hlink;clear. solve_addr. }
-    destruct rest as [|a l'];[inversion Hlength_rest|].
-    apply contiguous_between_cons_inv_first in Hcont_rest as Heq. subst.
-    (* move r_t5 r_t0 *)
-    destruct l';[inversion Hlength_rest|].
-    iPrologue "Hprog".
-    iApply (wp_move_success_reg with "[$HPC $Hi $Hr_t5 $Hr_t0]");
-      [apply decode_encode_instrW_inv|iCorrectLPC link a_last|iContiguous_next Hcont_rest 0|auto|..].
-    iEpilogue "(HPC & Hprog_done & Hr_t5 & Hr_t0)". iCombine "Hprog_done" "Hfetch" as "Hprog_done".
-    (* move r_t3 r_t1 *)
-    destruct l';[inversion Hlength_rest|].
-    iPrologue "Hprog".
-    iApply (wp_move_success_reg with "[$HPC $Hi $Hr_t3 $Hr_t1]");
-      [apply decode_encode_instrW_inv|iCorrectLPC link a_last|iContiguous_next Hcont_rest 1|auto|..].
-    iEpilogue "(HPC & Hi & Hr_t3 & Hr_t1)"; iCombine "Hi" "Hprog_done" as "Hprog_done".
-    (* move r_t1 size *)
-    destruct l';[inversion Hlength_rest|].
-    iPrologue "Hprog".
-    iApply (wp_move_success_z with "[$HPC $Hi $Hr_t1]");
-      [apply decode_encode_instrW_inv|iCorrectLPC link a_last|iContiguous_next Hcont_rest 2|auto|..].
-    iEpilogue "(HPC & Hi & Hr_t1)"; iCombine "Hi" "Hprog_done" as "Hprog_done".
-    (* move r_t0 PC *)
-    destruct l';[inversion Hlength_rest|].
-    iPrologue "Hprog".
-    iApply (wp_move_success_reg_fromPC with "[$HPC $Hi $Hr_t0]");
-      [apply decode_encode_instrW_inv|iCorrectLPC link a_last|iContiguous_next Hcont_rest 3|auto|..].
-    iEpilogue "(HPC & Hi & Hr_t0)"; iCombine "Hi" "Hprog_done" as "Hprog_done".
-    (* lea r_t0 3 *)
-    destruct l';[inversion Hlength_rest|]. destruct l';[inversion Hlength_rest|].
-    iPrologue "Hprog".
-    assert ((f1 + 3)%a = Some f4) as Hlea.
-    { apply (contiguous_between_incr_addr_middle _ _ _ 3 3 f1 f4) in Hcont_rest; auto. }
-    iApply (wp_lea_success_z with "[$HPC $Hi $Hr_t0]");
-      [apply decode_encode_instrW_inv|iCorrectLPC link a_last|iContiguous_next Hcont_rest 4|apply Hlea|auto..].
-    { apply contiguous_between_length in Hcont.
-      apply isCorrectPC_range_perm in Hvpc; [|revert Hcont; clear; solve_addr].
-      destruct Hvpc as [-> | -> ]; auto. }
-    iEpilogue "(HPC & Hi & Hr_t0)"; iCombine "Hi" "Hprog_done" as "Hprog_done".
-    (* jmp r_t3 *)
-    destruct l';[inversion Hlength_rest|].
-    iPrologue "Hprog".
-    iApply (wp_jmp_success with "[$HPC $Hi $Hr_t3]");
-      [apply decode_encode_instrW_inv|iCorrectLPC link a_last|].
-    iEpilogue "(HPC & Hi & Hr_t3) /="; iCombine "Hi" "Hprog_done" as "Hprog_done".
-    (* we are now ready to use the malloc subroutine spec. For this we prepare the registers *)
-    iDestruct (big_sepM_insert _ _ r_t3 with "[$Hregs $Hr_t3]") as "Hregs".
-      by rewrite lookup_delete_ne // lookup_delete.
-    iDestruct (big_sepM_insert _ _ r_t2 with "[$Hregs $Hr_t2]") as "Hregs".
-      by rewrite lookup_insert_ne // lookup_delete_ne // lookup_delete_ne // lookup_delete.
-    map_simpl "Hregs".
-    iDestruct (big_sepM_insert _ _ r_t5 with "[$Hregs $Hr_t5]") as "Hregs".
-      by simplify_map_eq. map_simpl "Hregs".
-    iApply (wp_wand with "[-]").
-    iApply (simple_malloc_subroutine_spec with "[- $Hmalloc $Hna $Hregs $Hr_t0 $HPC $Hr_t1]"); auto.
-    { rewrite !dom_insert_L dom_delete_L Hrmap_dom.
-      rewrite !difference_difference_l_L !singleton_union_difference_L !all_registers_union_l.
-      f_equal. }
-    (* { lia. } *)
-    iNext.
-    rewrite updatePcPermL_cap_non_E.
-    2: { eapply isCorrectPC_range_perm_non_E; eauto.
-         generalize (contiguous_between_length _ _ _ Hcont_rest). cbn.
-         clear; solve_addr. }
-    iIntros "((Hna & Hregs) & Hr_t0 & HPC & Hbe) /=".
-    iDestruct "Hbe" as (b e size' Hsize' Hbe) "(Hr_t1 & Hbe)". inversion Hsize'; subst size'.
-    iDestruct (big_sepM_delete _ _ r_t3 with "Hregs") as "[Hr_t3 Hregs]".
-      by rewrite lookup_insert_ne // lookup_insert //.
-      rewrite delete_insert_ne // delete_insert_delete.
-      repeat (rewrite delete_insert_ne //;[]). rewrite delete_insert_delete.
-    iDestruct (big_sepM_delete _ _ r_t5 with "Hregs") as "[Hr_t5 Hregs]".
-      by (repeat (rewrite lookup_insert_ne //;[]); rewrite lookup_insert //).
-      repeat (rewrite delete_insert_ne //;[]). rewrite delete_insert_delete.
-    (* move r_t0 r_t5 *)
-    iPrologue "Hprog".
-    iApply (wp_move_success_reg with "[$HPC $Hi $Hr_t0 $Hr_t5]");
-      [apply decode_encode_instrW_inv|iCorrectLPC link a_last|iContiguous_next Hcont_rest 6|auto|..].
-    iEpilogue "(HPC & Hi & Hr_t0 & Hr_t5)"; iCombine "Hi" "Hprog_done" as "Hprog_done".
-    (* move r_t5 0 *)
-    destruct l';[| by inversion Hlength_rest].
-    iPrologue "Hprog".
-    apply contiguous_between_last with (ai:=f5) in Hcont_rest as Hlast;[|auto].
-    iApply (wp_move_success_z with "[$HPC $Hi $Hr_t5]");
-      [apply decode_encode_instrW_inv|iCorrectLPC link a_last|apply Hlast|auto|..].
-    iEpilogue "(HPC & Hi & Hr_t5)"; iCombine "Hi" "Hprog_done" as "Hprog_done".
-    (* continuation *)
-    iApply "Hφ".
-    iFrame "HPC". iSplitL "Hprog_done".
-    { rewrite Heqapp. repeat (iDestruct "Hprog_done" as "[$ Hprog_done]"). iFrame. done. }
-    iFrame.
-    iDestruct (big_sepM_insert _ _ r_t5 with "[$Hregs $Hr_t5]") as "Hregs".
-      repeat (rewrite lookup_insert_ne //;[]). apply lookup_delete.
-    iDestruct (big_sepM_insert _ _ r_t3 with "[$Hregs $Hr_t3]") as "Hregs".
-      simplify_map_eq. auto.
-    repeat (rewrite (insert_commute _ r_t5) //;[]).
-    map_simpl "Hregs". rewrite (insert_commute _ r_t2 r_t3); auto.
-    iFrame.
-    iExists b,e. iFrame. auto. auto.
-  Qed.
-
-  (* malloc spec - alternative formulation *)
-  Lemma malloc_spec_alt φ ψ size cont a pc_p pc_b pc_e v a_first a_last
-        b_link e_link a_link f_m a_entry mallocN b_m e_m EN rmap :
-    isCorrectPC_range pc_p pc_b pc_e a_first a_last →
-    contiguous_between a a_first a_last →
-    withinBounds b_link e_link a_entry = true →
-    (a_link + f_m)%a = Some a_entry →
-    dom rmap = all_registers_s ∖ {[ PC; r_t0 ]} →
-    ↑mallocN ⊆ EN →
-    size > 0 →
-
-    (* malloc program and subroutine *)
-    ▷ malloc f_m size a v
-    ∗ na_inv logrel_nais mallocN (malloc_inv b_m e_m v)
-    ∗ na_own logrel_nais EN
-    (* we need to assume that the malloc capability is in the linking table at offset f_m *)
-    ∗ ▷ (pc_b,v) ↦ₐ LCap RO b_link e_link a_link v
-    ∗ ▷ (a_entry,v) ↦ₐ LCap E b_m e_m b_m v
-    (* register state *)
-    ∗ ▷ PC ↦ᵣ LCap pc_p pc_b pc_e a_first v
+    ∗ ▷ PC ↦ᵣ LCap pc_p pc_b pc_e a_first pc_v
     ∗ ▷ r_t0 ↦ᵣ cont
     ∗ ▷ ([∗ map] r_i↦w_i ∈ rmap, r_i ↦ᵣ w_i)
     (* failure/continuation *)
     ∗ ▷ (∀ v, ψ v -∗ φ v)
-    ∗ ▷ (ψ FailedV)
-    ∗ ▷ (PC ↦ᵣ LCap pc_p pc_b pc_e a_last v ∗ malloc f_m size a v
-         ∗ (pc_b,v) ↦ₐ LCap RO b_link e_link a_link v
-         ∗ (a_entry,v) ↦ₐ LCap E b_m e_m b_m v
+    ∗ ▷ (φ FailedV)
+    ∗ ▷ (PC ↦ᵣ LCap pc_p pc_b pc_e (a_first ^+ length (malloc_instrs f_m size))%a pc_v
+         ∗ codefrag a_first pc_v (malloc_instrs f_m size)
+         ∗ (pc_b,pc_v) ↦ₐ LCap RO b_link e_link a_link v_link
+         ∗ (a_entry,v_link) ↦ₐ LCap E b_m e_m b_m v_malloc
          (* the newly allocated region *)
          ∗ (∃ (b e : Addr),
             ⌜(b + size)%a = Some e⌝
-            ∗ r_t1 ↦ᵣ LCap RWX b e b v
-            ∗ [[b,e]] ↦ₐ{v} [[region_addrs_zeroesL b e v]])
+            ∗ r_t1 ↦ᵣ LCap RWX b e b v_malloc
+            ∗ [[b,e]] ↦ₐ{v_malloc} [[region_addrs_zeroesL b e v_malloc]])
          ∗ r_t0 ↦ᵣ cont
          ∗ na_own logrel_nais EN
          ∗ ([∗ map] r_i↦w_i ∈ (<[r_t2:=LInt 0%Z]>
@@ -534,1029 +317,566 @@ Section macros.
     iDestruct (big_sepM_delete _ _ r_t3 with "Hregs") as "[Hr_t3 Hregs]". by rewrite !lookup_delete_ne //.
     assert (is_Some (rmap !! r_t5)) as [rv5 ?]. by rewrite -elem_of_dom Hrmap_dom; set_solver.
     iDestruct (big_sepM_delete _ _ r_t5 with "Hregs") as "[Hr_t5 Hregs]". by rewrite !lookup_delete_ne //.
-    destruct a as [|a l];[inversion Hlength|].
-    apply contiguous_between_cons_inv_first in Hcont as Heq. subst.
-    (* fetch f *)
-    iDestruct ( (contiguous_betweenL_program_split _ _ (fun la w_i => la ↦ₐ w_i )%I) with "Hprog")
-      as (fetch_prog rest link) "(Hfetch & Hprog & #Hcont)";[apply Hcont|].
-    iDestruct "Hcont" as %(Hcont_fetch & Hcont_rest & Heqapp & Hlink).
-    iApply (fetch_spec with "[- $HPC $Hfetch $Hr_t1 $Hr_t2 $Hr_t3 $Ha_entry $Hpc_b]");
-      [|apply Hcont_fetch|apply Hwb|apply Ha_entry|].
-    { intros mid Hmid. apply isCorrectPC_inrange with a_first a_last; auto.
-      apply contiguous_between_bounds in Hcont_rest. revert Hcont_rest Hmid; clear. solve_addr. }
-    iNext. iIntros "(HPC & Hfetch& Hr_t1 & Hr_t2 & Hr_t3 & Hpc_b & Ha_entry)".
-    iDestruct (big_sepL2_length with "Hprog") as %Hlength_rest.
-    assert (isCorrectPC_range pc_p pc_b pc_e link a_last) as Hvpc_rest.
-    { intros mid Hmid. apply isCorrectPC_inrange with a_first a_last; auto. revert Hmid Hlink;clear. solve_addr. }
-    destruct rest as [|a l'];[inversion Hlength_rest|].
-    apply contiguous_between_cons_inv_first in Hcont_rest as Heq. subst.
-    (* move r_t5 r_t0 *)
-    destruct l';[inversion Hlength_rest|].
-    iPrologue "Hprog".
-    iApply (wp_move_success_reg with "[$HPC $Hi $Hr_t5 $Hr_t0]");
-      [apply decode_encode_instrW_inv|iCorrectLPC link a_last|iContiguous_next Hcont_rest 0|auto|..].
-    iEpilogue "(HPC & Hprog_done & Hr_t5 & Hr_t0)". iCombine "Hprog_done" "Hfetch" as "Hprog_done".
-    (* move r_t3 r_t1 *)
-    destruct l';[inversion Hlength_rest|].
-    iPrologue "Hprog".
-    iApply (wp_move_success_reg with "[$HPC $Hi $Hr_t3 $Hr_t1]");
-      [apply decode_encode_instrW_inv|iCorrectLPC link a_last|iContiguous_next Hcont_rest 1|auto|..].
-    iEpilogue "(HPC & Hi & Hr_t3 & Hr_t1)"; iCombine "Hi" "Hprog_done" as "Hprog_done".
-    (* move r_t1 size *)
-    destruct l';[inversion Hlength_rest|].
-    iPrologue "Hprog".
-    iApply (wp_move_success_z with "[$HPC $Hi $Hr_t1]");
-      [apply decode_encode_instrW_inv|iCorrectLPC link a_last|iContiguous_next Hcont_rest 2|auto|..].
-    iEpilogue "(HPC & Hi & Hr_t1)"; iCombine "Hi" "Hprog_done" as "Hprog_done".
-    (* move r_t0 PC *)
-    destruct l';[inversion Hlength_rest|].
-    iPrologue "Hprog".
-    iApply (wp_move_success_reg_fromPC with "[$HPC $Hi $Hr_t0]");
-      [apply decode_encode_instrW_inv|iCorrectLPC link a_last|iContiguous_next Hcont_rest 3|auto|..].
-    iEpilogue "(HPC & Hi & Hr_t0)"; iCombine "Hi" "Hprog_done" as "Hprog_done".
-    (* lea r_t0 3 *)
-    destruct l';[inversion Hlength_rest|]. destruct l';[inversion Hlength_rest|].
-    iPrologue "Hprog".
-    assert ((f1 + 3)%a = Some f4) as Hlea.
-    { apply (contiguous_between_incr_addr_middle _ _ _ 3 3 f1 f4) in Hcont_rest; auto. }
-    iApply (wp_lea_success_z with "[$HPC $Hi $Hr_t0]");
-      [apply decode_encode_instrW_inv|iCorrectLPC link a_last|iContiguous_next Hcont_rest 4|apply Hlea|auto..].
-    { apply contiguous_between_length in Hcont.
-      apply isCorrectPC_range_perm in Hvpc; [|revert Hcont; clear; solve_addr].
-      destruct Hvpc as [-> | -> ]; auto. }
-    iEpilogue "(HPC & Hi & Hr_t0)"; iCombine "Hi" "Hprog_done" as "Hprog_done".
-    (* jmp r_t3 *)
-    destruct l';[inversion Hlength_rest|].
-    iPrologue "Hprog".
-    iApply (wp_jmp_success with "[$HPC $Hi $Hr_t3]");
-      [apply decode_encode_instrW_inv|iCorrectLPC link a_last|].
-    iEpilogue "(HPC & Hi & Hr_t3) /="; iCombine "Hi" "Hprog_done" as "Hprog_done".
+
+    rewrite {1}/malloc_instrs.
+    focus_block_0 "Hprog" as "Hfetch" "Hcont".
+    iApply fetch_spec; iFrameAutoSolve.
+    iNext. iIntros "(HPC & Hfetch & Hr_t1 & Hr_t2 & Hr_t3 & Hpc_b & Ha_entry)".
+    unfocus_block "Hfetch" "Hcont" as "Hprog".
+
+    focus_block 1 "Hprog" as amid1 Hamid1 "Hprog" "Hcont".
+    iGo "Hprog". (* PC is now at b_m *)
     (* we are now ready to use the malloc subroutine spec. For this we prepare the registers *)
     iDestruct (big_sepM_insert _ _ r_t3 with "[$Hregs $Hr_t3]") as "Hregs".
-      by rewrite lookup_delete_ne // lookup_delete.
+      by simplify_map_eq.
     iDestruct (big_sepM_insert _ _ r_t2 with "[$Hregs $Hr_t2]") as "Hregs".
-      by rewrite lookup_insert_ne // lookup_delete_ne // lookup_delete_ne // lookup_delete.
-    rewrite -(delete_insert_ne _ r_t5 r_t3) // insert_delete_insert.
-    rewrite -(delete_insert_ne _ r_t5 r_t2) //.
-    rewrite (insert_commute ((delete r_t2 _)) r_t2 r_t3) //.
-    rewrite insert_delete_insert.
+      by simplify_map_eq.
+    map_simpl "Hregs".
     iDestruct (big_sepM_insert _ _ r_t5 with "[$Hregs $Hr_t5]") as "Hregs".
-      by rewrite lookup_delete. rewrite insert_delete_insert.
+      by simplify_map_eq.
+    map_simpl "Hregs".
     iApply (wp_wand with "[- Hφfailed Hψ]").
     iApply (simple_malloc_subroutine_spec with "[- $Hmalloc $Hna $Hregs $Hr_t0 $HPC $Hr_t1]"); auto.
-    { rewrite !dom_insert_L dom_delete_L Hrmap_dom.
-      rewrite !difference_difference_l_L !singleton_union_difference_L !all_registers_union_l.
-      f_equal. }
-    (* { lia. } *)
+    { set_solver+ Hrmap_dom. }
     iNext.
-    rewrite updatePcPermL_cap_non_E.
-    2: { eapply isCorrectPC_range_perm_non_E; eauto.
-         generalize (contiguous_between_length _ _ _ Hcont_rest). cbn.
-         clear; solve_addr. }
+    rewrite updatePcPermL_cap_non_E; [| solve_pure].
     iIntros "((Hna & Hregs) & Hr_t0 & HPC & Hbe) /=".
-    iDestruct "Hbe" as (b e size' Hsize' Hbe) "(Hr_t1 & Hbe)". inversion Hsize';subst size'.
+    iDestruct "Hbe" as (b e size' Hsize' Hbe) "(Hr_t1 & Hbe)". inversion Hsize'; subst size'.
     iDestruct (big_sepM_delete _ _ r_t3 with "Hregs") as "[Hr_t3 Hregs]".
-      by rewrite lookup_insert_ne // lookup_insert //.
-      rewrite delete_insert_ne // delete_insert_delete.
-      repeat (rewrite delete_insert_ne //;[]). rewrite delete_insert_delete.
+      simplify_map_eq. eauto.
     iDestruct (big_sepM_delete _ _ r_t5 with "Hregs") as "[Hr_t5 Hregs]".
-      by (repeat (rewrite lookup_insert_ne //;[]); rewrite lookup_insert //).
-      repeat (rewrite delete_insert_ne //;[]). rewrite delete_insert_delete.
-    (* move r_t0 r_t5 *)
-    iPrologue "Hprog".
-    iApply (wp_move_success_reg with "[$HPC $Hi $Hr_t0 $Hr_t5]");
-      [apply decode_encode_instrW_inv|iCorrectLPC link a_last|iContiguous_next Hcont_rest 6|auto|..].
-    iEpilogue "(HPC & Hi & Hr_t0 & Hr_t5)"; iCombine "Hi" "Hprog_done" as "Hprog_done".
-    (* move r_t5 0 *)
-    destruct l';[| by inversion Hlength_rest].
-    iPrologue "Hprog".
-    apply contiguous_between_last with (ai:=f5) in Hcont_rest as Hlast;[|auto].
-    iApply (wp_move_success_z with "[$HPC $Hi $Hr_t5]");
-      [apply decode_encode_instrW_inv|iCorrectLPC link a_last|apply Hlast|auto|..].
-    iEpilogue "(HPC & Hi & Hr_t5)"; iCombine "Hi" "Hprog_done" as "Hprog_done".
+      simplify_map_eq. eauto.
+    (* back our program, in the continuation of malloc *)
+    iGo "Hprog".
+    unfocus_block "Hprog" "Hcont" as "Hprog".
     (* continuation *)
-    iApply "Hφ".
-    iFrame "HPC". iSplitL "Hprog_done".
-    { rewrite Heqapp. repeat (iDestruct "Hprog_done" as "[$ Hprog_done]"). iFrame. done. }
-    iFrame.
-    iDestruct (big_sepM_insert _ _ r_t5 with "[$Hregs $Hr_t5]") as "Hregs".
-      repeat (rewrite lookup_insert_ne //;[]). apply lookup_delete.
-    iDestruct (big_sepM_insert _ _ r_t3 with "[$Hregs $Hr_t3]") as "Hregs".
-      repeat (rewrite lookup_insert_ne //;[]).
-      rewrite lookup_delete_ne // lookup_delete //.
-    repeat (rewrite (insert_commute _ r_t5) //;[]).
-    rewrite insert_delete_insert -(delete_insert_ne _ _ r_t5) //.
-    rewrite (insert_commute _ r_t5 r_t2) // (delete_insert_ne _ r_t3 r_t2)//.
-    rewrite (insert_commute _ r_t4 r_t2) // insert_insert.
-    rewrite (insert_commute _ r_t3 r_t2) //.
-    rewrite -(delete_insert_ne _ r_t3) // insert_delete_insert.
-    iFrame.
-    iExists b,e. iFrame. auto. iIntros (w) "[Hφ|Hφ] /=". iApply "Hψ". iFrame. iSimplifyEq. iApply "Hψ". iFrame.
+    iApply "Hφ". changePCto (a_first ^+ 18%nat)%a.
+    iFrame. iSplitL "Hr_t1 Hbe".
+    { iExists _,_. iFrame. iPureIntro; eauto. }
+    { iDestruct (big_sepM_insert _ _ r_t5 with "[$Hregs $Hr_t5]") as "Hregs".
+        simplify_map_eq. reflexivity.
+      iDestruct (big_sepM_insert _ _ r_t3 with "[$Hregs $Hr_t3]") as "Hregs".
+      simplify_map_eq. reflexivity.
+      iFrameMapSolve+ Hrmap_dom "Hregs". }
+    { iIntros (w) "[Hφ|Hφ] /=". iApply "Hψ". iFrame. iSimplifyEq. eauto. }
   Qed.
 
+  (* malloc spec - alternative formulation *)
+  Lemma malloc_spec φ size cont pc_p pc_b pc_e pc_v a_first
+        b_link e_link a_link v_link f_m a_entry v_malloc mallocN b_m e_m EN rmap :
+    ExecPCPerm pc_p →
+    SubBounds pc_b pc_e a_first (a_first ^+ length (malloc_instrs f_m size))%a →
+    withinBounds b_link e_link a_entry = true →
+    (a_link + f_m)%a = Some a_entry →
+    dom rmap = all_registers_s ∖ {[ PC; r_t0 ]} →
+    ↑mallocN ⊆ EN →
+    (size > 0)%Z →
 
-  (* -------------------------------------- RCLEAR ----------------------------------- *)
-  (* the following macro clears registers in r. a denotes the list of addresses
-     containing the instructions for the clear: |a| = |r| *)
-  Definition rclear_instrs (r : list RegName) := map (λ r_i, encodeInstrWL (Mov r_i 0)) r.
-
-  Lemma rclear_instrs_cons rr r: rclear_instrs (rr :: r) = (encodeInstrWL (Mov rr 0)):: rclear_instrs r.
-  Proof. reflexivity. Qed.
-
-  Definition rclear (a : list Addr) (r : list RegName) v : iProp Σ :=
-      ([∗ list] k↦a_i;w_i ∈ a;(rclear_instrs r), (a_i,v) ↦ₐ w_i)%I.
-
-  Lemma rclear_spec (a : list Addr) (r: list RegName) (rmap : gmap RegName LWord) p b e a1 an v φ :
-    contiguous_between a a1 an →
-    ¬ PC ∈ r → hd_error a = Some a1 →
-    isCorrectPC_range p b e a1 an →
-    list_to_set r = dom rmap →
-
-      ▷ ([∗ map] r_i↦w_i ∈ rmap, r_i ↦ᵣ w_i)
-    ∗ ▷ PC ↦ᵣ LCap p b e a1 v
-    ∗ ▷ rclear a r v
-    ∗ ▷ (PC ↦ᵣ LCap p b e an v ∗ ([∗ map] r_i↦_ ∈ rmap, r_i ↦ᵣ LInt 0%Z)
-            ∗ rclear a r v -∗
-            WP Seq (Instr Executable) {{ φ }})
-    ⊢ WP Seq (Instr Executable) {{ φ }}.
+    (* malloc program and subroutine *)
+    ▷ codefrag a_first pc_v (malloc_instrs f_m size)
+    ∗ na_inv logrel_nais mallocN (malloc_inv b_m e_m v_malloc)
+    ∗ na_own logrel_nais EN
+    (* we need to assume that the malloc capability is in the linking table at offset f_m *)
+    ∗ ▷ (pc_b,pc_v) ↦ₐ LCap RO b_link e_link a_link v_link
+    ∗ ▷ (a_entry,v_link) ↦ₐ LCap E b_m e_m b_m v_malloc
+    (* register state *)
+    ∗ ▷ PC ↦ᵣ LCap pc_p pc_b pc_e a_first pc_v
+    ∗ ▷ r_t0 ↦ᵣ cont
+    ∗ ▷ ([∗ map] r_i↦w_i ∈ rmap, r_i ↦ᵣ w_i)
+    (* continuation *)
+    ∗ ▷ (PC ↦ᵣ LCap pc_p pc_b pc_e (a_first ^+ length (malloc_instrs f_m size))%a pc_v
+         ∗ codefrag a_first pc_v (malloc_instrs f_m size)
+         ∗ (pc_b,pc_v) ↦ₐ LCap RO b_link e_link a_link v_link
+         ∗ (a_entry,v_link) ↦ₐ LCap E b_m e_m b_m v_malloc
+         (* the newly allocated region *)
+         ∗ (∃ (b e : Addr),
+            ⌜(b + size)%a = Some e⌝
+            ∗ r_t1 ↦ᵣ LCap RWX b e b v_malloc
+            ∗ [[b,e]] ↦ₐ{v_malloc} [[region_addrs_zeroesL b e v_malloc]])
+         ∗ r_t0 ↦ᵣ cont
+         ∗ na_own logrel_nais EN
+         ∗ ([∗ map] r_i↦w_i ∈ (<[r_t2:=LInt 0%Z]>
+                               (<[r_t3:=LInt 0%Z]>
+                                (<[r_t4:=LInt 0%Z]>
+                                 (<[r_t5:=LInt 0%Z]> (delete r_t1 rmap))))), r_i ↦ᵣ w_i)
+         (* the newly allocated region is fresh in the current world *)
+         (* ∗ ⌜Forall (λ a, a ∉ dom (gset Addr) (std W)) (finz.seq_between b e)⌝ *)
+         -∗ WP Seq (Instr Executable) {{ φ }})
+    ⊢
+      WP Seq (Instr Executable) {{ λ v, φ v ∨ ⌜v = FailedV⌝ }}.
   Proof.
-    iIntros (Ha Hne Hhd Hvpc Hrdom) "(>Hreg & >HPC & >Hrclear & Hφ)".
-    iDestruct (big_sepL2_length with "Hrclear") as %Har.
-    iRevert (Hne Har Hhd Hvpc Ha Hrdom).
-    iInduction (a) as [| a1'] "IH" forall (r rmap a1 an).
-    { iIntros (Hne Har Hhd Hvpc Ha Hrdom). by inversion Hhd; simplify_eq. }
-    iIntros (Hne Har Hhd Hvpc Ha Hrdom).
-    iApply (wp_bind (fill [SeqCtx])). rewrite /rclear /=.
-    (* rewrite -(beq_nat_refl (length r)).  *)destruct r; inversion Har.
-    rewrite rclear_instrs_cons.
-    iDestruct (big_sepL2_cons with "Hrclear") as "[Ha1 Hrclear]".
-    rewrite list_to_set_cons in Hrdom.
-    assert (is_Some (rmap !! r)) as [rv ?].
-    { rewrite -elem_of_dom -Hrdom. set_solver. }
-    iDestruct (big_sepM_delete _ _ r with "Hreg") as "[Hr Hreg]". eauto.
-    pose proof (contiguous_between_cons_inv _ _ _ _ Ha) as [-> [a2 [? Hcont'] ] ].
-    iApply (wp_move_success_z with "[$HPC $Hr $Ha1]");
-      [apply decode_encode_instrW_inv|iCorrectLPC a1 an|eauto|..].
-    iNext. iIntros "(HPC & Ha1 & Hr)". iApply wp_pure_step_later; auto.
-    iNext; iIntros "_".
-    destruct a.
-    { iApply "Hφ". iFrame. inversion Hcont'; subst. iFrame.
-      destruct r0; inversion Har. simpl in Hrdom.
-      iApply (big_sepM_delete _ _ r). eauto.
-      rewrite (_: delete r rmap = ∅). rewrite !big_sepM_empty. eauto.
-      apply map_empty. intro. eapply (@not_elem_of_dom _ _ (gset RegName)).
-      typeclasses eauto. rewrite dom_delete_L -Hrdom. set_solver. }
-
-    pose proof (contiguous_between_cons_inv_first _ _ _ _ Hcont') as ->.
-    assert (PC ∉ r0). { apply not_elem_of_cons in Hne as [? ?]. auto. }
-
-    destruct (decide (r ∈ r0)).
-    { iDestruct (big_sepM_insert with "[$Hreg $Hr]") as "Hreg".
-        by rewrite lookup_delete. rewrite insert_delete_insert.
-      iApply ("IH" with "Hreg HPC Hrclear [Hφ Ha1]"); eauto.
-      { iNext. iIntros "(? & Hreg & ?)". iApply "Hφ". iFrame.
-        iApply (big_sepM_delete _ _ r). eauto.
-        iDestruct (big_sepM_delete _ _ r with "Hreg") as "[? ?]".
-        rewrite lookup_insert //. iFrame. rewrite delete_insert_delete //. }
-      { iPureIntro. intros ? [? ?]. apply Hvpc. solve_addr. }
-      { iPureIntro. rewrite dom_insert_L -Hrdom. set_solver. } }
-    { iApply ("IH" with "Hreg HPC Hrclear [Hφ Ha1 Hr]"); eauto.
-      { iNext. iIntros "(? & ? & ?)". iApply "Hφ". iFrame.
-        iApply (big_sepM_delete _ _ r). eauto. iFrame. }
-      { iPureIntro. intros ? [? ?]. apply Hvpc. solve_addr. }
-      { iPureIntro. rewrite dom_delete_L -Hrdom. set_solver. } }
+    iIntros (Hvpc Hcont Hwb Ha_entry Hrmap_dom HmallocN Hsize)
+            "(>Hprog & #Hmalloc & Hna & >Hpc_b & >Ha_entry & >HPC & >Hr_t0 & >Hregs & Hφ)".
+    iApply malloc_spec_alt; iFrameAutoSolve; eauto. iFrame. iFrame "Hmalloc".
+    iSplitL. iNext. eauto. eauto.
   Qed.
 
-  (* -------------------------------------- MCLEAR ----------------------------------- *)
-   (* the following macro clears the region of memory a capability govers over. a denotes
-     the list of adresses containing the instructions for the clear. |a| = 23 *)
+  (* --------------------------------------------------------------------------------- *)
+  (* ------------------------------------- SALLOC ------------------------------------ *)
+  (* --------------------------------------------------------------------------------- *)
 
-  Definition mclear_off_end := 10%Z.
-  Definition mclear_off_iter := 2%Z.
+  (* salloc stores the result in r_t1, rather than a user chosen destination.
+     f_m is the offset of the salloc capability *)
+  (* Definition salloc_instrs f_m (size: Z) := *)
+  (*   fetch_instrs f_m ++ *)
+  (*   encodeInstrsLW [ *)
+  (*    Mov r_t5 r_t0; *)
+  (*    Mov r_t3 r_t1; *)
+  (*    Mov r_t1 size; *)
+  (*    Mov r_t0 PC; *)
+  (*    Lea r_t0 3; *)
+  (*    Jmp r_t3; *)
+  (*    Mov r_t0 r_t5; *)
+  (*    Mov r_t5 0 *)
+  (* ]. *)
 
-  (* first we will define the list of Words making up the mclear macro *)
-  Definition mclear_instrs r_stk :=
-    encodeInstrsLW [
-        Mov r_t4 r_stk;
-        GetB r_t1 r_t4;
-        GetA r_t2 r_t4;
-        Sub r_t2 r_t1 r_t2;
-        Lea r_t4 r_t2;
-        GetE r_t5 r_t4;
-        Sub r_t5 r_t5 1; (* we subtract the bound by one so that the lt check becomes a le check *)
-        Mov r_t2 PC;
-        Lea r_t2 mclear_off_end; (* offset to "end" *)
-        Mov r_t3 PC;
-        Lea r_t3 mclear_off_iter; (* offset to "iter" *)
-        (* iter: *)
-        Lt r_t6 r_t5 r_t1;
-        Jnz r_t2 r_t6;
-        Store r_t4 0;
-        Lea r_t4 1;
-        Add r_t1 r_t1 1;
-        Jmp r_t3;
-        (* end: *)
-        Mov r_t4 0;
-        Mov r_t1 0;
-        Mov r_t2 0;
-        Mov r_t3 0;
-        Mov r_t5 0;
-        Mov r_t6 0].
+  (* (* salloc spec *) *)
+  (* Lemma salloc_spec_alt φ ψ size cont pc_p pc_b pc_e v a_first *)
+  (*       b_link e_link a_link f_m a_entry sallocN b_m e_m EN rmap : *)
+  (*   ExecPCPerm pc_p → *)
+  (*   SubBounds pc_b pc_e a_first (a_first ^+ length (salloc_instrs f_m size))%a → *)
+  (*   withinBounds b_link e_link a_entry = true → *)
+  (*   (a_link + f_m)%a = Some a_entry → *)
+  (*   dom rmap = all_registers_s ∖ {[ PC; r_t0 ]} → *)
+  (*   ↑sallocN ⊆ EN → *)
+  (*   (size > 0)%Z → *)
 
-  (* Next we define mclear in memory, using a list of addresses of size 23 *)
-  Definition mclear (a : list Addr) (r : RegName) (v : Version) : iProp Σ :=
-    if ((length a) =? (length (mclear_instrs r)))%nat then
-      ([∗ list] k↦a_i;w_i ∈ a;(mclear_instrs r), (a_i, v) ↦ₐ w_i)%I
-    else
-      False%I.
+  (*   (* salloc program and subroutine *) *)
+  (*   ▷ codefrag a_first v (salloc_instrs f_m size) *)
+  (*   ∗ na_inv logrel_nais sallocN (salloc_inv b_m e_m v) *)
+  (*   ∗ na_own logrel_nais EN *)
+  (*   (* we need to assume that the salloc capability is in the linking table at offset f_m *) *)
+  (*   ∗ ▷ (pc_b,v) ↦ₐ LCap RO b_link e_link a_link v *)
+  (*   ∗ ▷ (a_entry,v) ↦ₐ LCap E b_m e_m b_m v *)
+  (*   (* register state *) *)
+  (*   ∗ ▷ PC ↦ᵣ LCap pc_p pc_b pc_e a_first v *)
+  (*   ∗ ▷ r_t0 ↦ᵣ cont *)
+  (*   ∗ ▷ ([∗ map] r_i↦w_i ∈ rmap, r_i ↦ᵣ w_i) *)
+  (*   (* failure/continuation *) *)
+  (*   ∗ ▷ (∀ v, ψ v -∗ φ v) *)
+  (*   ∗ ▷ (φ FailedV) *)
+  (*   ∗ ▷ (PC ↦ᵣ LCap pc_p pc_b pc_e (a_first ^+ length (salloc_instrs f_m size))%a v *)
+  (*        ∗ codefrag a_first v (salloc_instrs f_m size) *)
+  (*        ∗ (pc_b,v) ↦ₐ LCap RO b_link e_link a_link v *)
+  (*        ∗ (a_entry,v) ↦ₐ LCap E b_m e_m b_m v *)
+  (*        (* the newly allocated region *) *)
+  (*        ∗ (∃ (bs es : OType), *)
+  (*           ⌜(bs + size)%ot = Some es⌝ *)
+  (*           ∗ r_t1 ↦ᵣ LSealRange (true,true) bs es bs *)
+  (*           ∗ ([∗ list] o ∈ finz.seq_between bs es, can_alloc_pred o)) *)
+  (*        ∗ r_t0 ↦ᵣ cont *)
+  (*        ∗ na_own logrel_nais EN *)
+  (*        ∗ ([∗ map] r_i↦w_i ∈ (<[r_t2:=LInt 0%Z]> *)
+  (*                              (<[r_t3:=LInt 0%Z]> *)
+  (*                               (<[r_t4:=LInt 0%Z]> *)
+  (*                                (<[r_t5:=LInt 0%Z]> (delete r_t1 rmap))))), r_i ↦ᵣ w_i) *)
+  (*        (* the newly allocated region is fresh in the current world *) *)
+  (*        (* ∗ ⌜Forall (λ a, a ∉ dom (gset Addr) (std W)) (finz.seq_between b e)⌝ *) *)
+  (*        -∗ WP Seq (Instr Executable) {{ ψ }}) *)
+  (*   ⊢ *)
+  (*     WP Seq (Instr Executable) {{ λ v, φ v }}. *)
+  (* Proof. *)
+  (*   iIntros (Hvpc Hcont Hwb Ha_entry Hrmap_dom HsallocN Hsize) *)
+  (*           "(>Hprog & #Hsalloc & Hna & >Hpc_b & >Ha_entry & >HPC & >Hr_t0 & >Hregs & Hψ & Hφfailed & Hφ)". *)
+  (*   (* extract necessary registers from regs *) *)
+  (*   iDestruct (big_sepL2_length with "Hprog") as %Hlength. *)
+  (*   assert (is_Some (rmap !! r_t1)) as [rv1 ?]. by rewrite -elem_of_dom Hrmap_dom; set_solver. *)
+  (*   iDestruct (big_sepM_delete _ _ r_t1 with "Hregs") as "[Hr_t1 Hregs]"; eauto. *)
+  (*   assert (is_Some (rmap !! r_t2)) as [rv2 ?]. by rewrite -elem_of_dom Hrmap_dom; set_solver. *)
+  (*   iDestruct (big_sepM_delete _ _ r_t2 with "Hregs") as "[Hr_t2 Hregs]". by rewrite lookup_delete_ne //. *)
+  (*   assert (is_Some (rmap !! r_t3)) as [rv3 ?]. by rewrite -elem_of_dom Hrmap_dom; set_solver. *)
+  (*   iDestruct (big_sepM_delete _ _ r_t3 with "Hregs") as "[Hr_t3 Hregs]". by rewrite !lookup_delete_ne //. *)
+  (*   assert (is_Some (rmap !! r_t5)) as [rv5 ?]. by rewrite -elem_of_dom Hrmap_dom; set_solver. *)
+  (*   iDestruct (big_sepM_delete _ _ r_t5 with "Hregs") as "[Hr_t5 Hregs]". by rewrite !lookup_delete_ne //. *)
 
-  Lemma mclear_iter_spec (a1 a2 a3 a4 a5 a6 b_r e_r a_r (* e_r' *) : Addr) v ws (z : nat)
-        p b e rt rt1 rt2 rt3 rt4 rt5 a_end (p_r : Perm) φ :
-        isCorrectLPC (LCap p b e a1 v)
-      ∧ isCorrectLPC (LCap p b e a2 v)
-      ∧ isCorrectLPC (LCap p b e a3 v)
-      ∧ isCorrectLPC (LCap p b e a4 v)
-      ∧ isCorrectLPC (LCap p b e a5 v)
-      ∧ isCorrectLPC (LCap p b e a6 v) →
-        (a1 + 1)%a = Some a2
-      ∧ (a2 + 1)%a = Some a3
-      ∧ (a3 + 1)%a = Some a4
-      ∧ (a4 + 1)%a = Some a5
-      ∧ (a5 + 1)%a = Some a6 →
-        ((b_r + z < e_r)%Z → withinBounds b_r e_r a_r = true) →
-        writeAllowed p_r = true →
-        (* (e_r + 1)%a = Some e_r' → *)
-        (b_r + z)%a = Some a_r →
-      ([[a_r,e_r]] ↦ₐ{v} [[ws]]
-     ∗ ▷ PC ↦ᵣ LCap p b e a1 v
-     ∗ ▷ rt ↦ᵣ LCap p_r b_r e_r a_r v
-     ∗ ▷ rt1 ↦ᵣ LInt (b_r + z)%Z
-     ∗ ▷ rt2 ↦ᵣ LInt ((z_of e_r) - 1)%Z
-     ∗ ▷ (∃ w, rt3 ↦ᵣ w)
-     ∗ ▷ rt4 ↦ᵣ LCap p b e a_end v
-     ∗ ▷ rt5 ↦ᵣ LCap p b e a1 v
-     ∗ ▷ ([∗ list] a_i;w_i ∈ [a1;a2;a3;a4;a5;a6];
-          (encodeInstrsLW
-             [Lt rt3 rt2 rt1;
-              Jnz rt4 rt3;
-              Store rt 0;
-              Lea rt 1;
-              Add rt1 rt1 1;
-              Jmp rt5]
-          ) , (a_i,v) ↦ₐ w_i)
-     ∗ ▷ (PC ↦ᵣ updatePcPermL (LCap p b e a_end v)
-             ∗ [[ a_r , e_r ]] ↦ₐ{v} [[ region_addrs_zeroesL a_r e_r v ]]
-             ∗ (∃ a_r, rt ↦ᵣ LCap p_r b_r e_r a_r v)
-             ∗ rt5 ↦ᵣ LCap p b e a1 v
-             ∗ (a3,v) ↦ₐ (encodeInstrWL (Store rt 0))
-             ∗ (a4,v) ↦ₐ (encodeInstrWL (Lea rt 1))
-             ∗ (a5,v) ↦ₐ (encodeInstrWL (Add rt1 rt1 1))
-             ∗ (a6,v) ↦ₐ (encodeInstrWL (Jmp rt5))
-             ∗ (a1,v) ↦ₐ (encodeInstrWL (Lt rt3 rt2 rt1))
-             ∗ rt2 ↦ᵣ LInt ((z_of e_r) - 1)%Z
-             ∗ (∃ z, rt1 ↦ᵣ LInt (b_r + z)%Z)
-             ∗ (a2,v) ↦ₐ (encodeInstrWL (Jnz rt4 rt3))
-             ∗ rt4 ↦ᵣ LCap p b e a_end v
-             ∗ rt3 ↦ᵣ LInt 1%Z
-              -∗ WP Seq (Instr Executable) {{ φ }})
-     ⊢ WP Seq (Instr Executable) {{ φ }})%I.
-  Proof.
-    iIntros (Hvpc Hnext Hwb Hwa (* Her' *) Hprogress)
-            "(Hbe & >HPC & >Hrt & >Hr_t1 & >Hr_t2 & >Hr_t3 & >Hr_t4 & >Hr_t5 & >Hprog & Hφ)".
-    iRevert (Hwb Hprogress).
-    iLöb as "IH" forall (a_r ws z).
-    iIntros (Hwb Hprogress).
-    iDestruct "Hr_t3" as (w) "Hr_t3".
-    destruct Hvpc as (Hvpc1 & Hvpc2 & Hvpc3 & Hvpc4 & Hvpc5 & Hvpc6).
-    destruct Hnext as (Hnext1 & Hnext2 & Hnext3 & Hnext4 & Hnext5).
-    iAssert (⌜rt1 ≠ PC⌝)%I as %Hne1.
-    { destruct (reg_eq_dec rt1 PC); auto. rewrite e0.
-        by iDestruct (regname_dupl_false with "Hr_t1 HPC") as "Hfalse". }
-    iAssert (⌜rt3 ≠ PC⌝)%I as %Hne2.
-    { destruct (reg_eq_dec rt3 PC); auto. rewrite e0.
-        by iDestruct (regname_dupl_false with "Hr_t3 HPC") as "Hfalse". }
-    iAssert (⌜rt ≠ PC⌝)%I as %Hne3.
-    { destruct (reg_eq_dec rt PC); auto. rewrite e0.
-        by iDestruct (regname_dupl_false with "Hrt HPC") as "Hfalse". }
-    iAssert (⌜rt2 ≠ rt3⌝)%I as %Hne4.
-    { destruct (reg_eq_dec rt2 rt3); auto. rewrite e0.
-        by iDestruct (regname_dupl_false with "Hr_t2 Hr_t3") as "Hfalse". }
-    iAssert (⌜rt1 ≠ rt3⌝)%I as %Hne5.
-    { destruct (reg_eq_dec rt1 rt3); auto. rewrite e0.
-        by iDestruct (regname_dupl_false with "Hr_t1 Hr_t3") as "Hfalse". }
-    (* lt rt3 rt2 rt1 *)
-    iDestruct "Hprog" as "[Hi Hprog]".
-    iApply (wp_bind (fill [SeqCtx])).
-    iApply (wp_add_sub_lt_success_r_r _ rt3 _ _ _ a1 _ _ _  _ rt2 _ rt1 _ _
-      with "[Hi HPC Hr_t3 Hr_t1 Hr_t2]"); [apply decode_encode_instrLW_inv | | | | iFrame | ..]
-    ; eauto.
-    iFrame.
-    iEpilogue "(HPC & Ha1 & Hr_t2 & Hr_t1 & Hr_t3)".
-    rewrite /region_mapsto /finz.seq_between.
-    destruct (Z.le_dec (b_r + z) (e_r - 1))%Z; simpl.
-    - assert (Z.b2z (e_r - 1 <? b_r + z)%Z = 0%Z) as Heq0.
-      { rewrite /Z.b2z. destruct (e_r - 1 <? b_r + z)%Z eqn:HH; auto.
-        apply Z.ltb_lt in HH. lia. }
-      rewrite Heq0.
-      (* jnz rt4 rt3 *)
-      iDestruct "Hprog" as "[Hi Hprog]".
-      iApply (wp_bind (fill [SeqCtx])).
-      iApply (wp_jnz_success_next _ rt4 rt3 _ _ _ a2 _ a3 with "[HPC Hi Hr_t3 Hr_t4]");
-        first apply decode_encode_instrLW_inv; eauto.
-      iFrame. iEpilogue "(HPC & Ha2 & Hr_t4 & Hr_t3)".
-      (* store rt 0 *)
-      rewrite/ withinBounds in Hwb.
-      apply andb_prop in Hwb as [Hwb_b%Z.leb_le Hwb_e%Z.ltb_lt].
-      rewrite {1}finz_dist_S /=.
-      destruct ws as [| w1 ws]; simpl; [by iApply bi.False_elim|].
-      iDestruct "Hbe" as "[Ha_r Hbe]".
-      iDestruct "Hprog" as "[Hi Hprog]".
-      iApply (wp_bind (fill [SeqCtx])).
-      iApply (wp_store_success_z _ _ _ _  a3 _ a4 _ rt 0 _ p_r b_r e_r a_r with "[HPC Hi Hrt Ha_r]"); first apply decode_encode_instrLW_inv; eauto.
-      { rewrite /withinBounds andb_true_iff; split;[auto|].
-          by apply Z.leb_le. by apply Z.ltb_lt. }
-      iFrame. iEpilogue "(HPC & Ha3 & Hrt & Ha_r)".
-      (* lea rt 1 *)
-      assert (∃ a_r', (a_r + 1)%a = Some a_r') as [a_r' Ha_r'].
-      { apply addr_next_lt with e_r. apply incr_addr_of_z_i in Hprogress. lia. }
-      iDestruct "Hprog" as "[Hi Hprog]".
-      iApply (wp_bind (fill [SeqCtx])).
-      iApply (wp_lea_success_z _ _ _ _ a4 a5 _ _ rt p_r _ _ a_r _ 1 a_r' with "[HPC Hi Hrt]"); first apply decode_encode_instrLW_inv; eauto.
-      { destruct p_r; auto. }
-      iFrame. iEpilogue "(HPC & Ha4 & Hrt)".
-      (* add rt1 rt1 1 *)
-      iDestruct "Hprog" as "[Hi Hprog]".
-      iApply (wp_bind (fill [SeqCtx])).
-      iApply (wp_add_sub_lt_success_dst_z _ rt1 _ _ _ a5 _ _ _ with "[HPC Hi Hr_t1]"); try iFrame;
-        [ apply decode_encode_instrW_inv | | |..]; eauto.
-      iEpilogue "(HPC & Ha5 & Hr_t1)".
-      (* jmp rt5 *)
-      iDestruct "Hprog" as "[Hi _]".
-      iApply (wp_bind (fill [SeqCtx])).
-      iApply (wp_jmp_success _ _ _ _ a6 with "[HPC Hi Hr_t5]");
-        first apply decode_encode_instrLW_inv; eauto.
-      iFrame. iEpilogue "(HPC & Ha6 & Hr_t5)".
-      iApply ("IH" $! a_r' ws (z + 1)%nat with
-                  "[Hbe] [HPC] [Hrt] [Hr_t1] [Hr_t2] [Hr_t3] [Hr_t4] [Hr_t5] [Ha1 Ha2 Ha3 Ha4 Ha5 Ha6] [Hφ Ha_r]")
-      ; iFrame. all: auto.
-      + by rewrite (addr_incr_eq Ha_r').
-      + assert (updatePcPermL (LCap p b e a1 v) = (LCap p b e a1 v)).
-        { rewrite /updatePcPermL. destruct p; auto.
-          inversion Hvpc1;inversion H0; cbn in * ; simplify_eq; destruct H7 as [Hc | Hc ]; inversion Hc. }
-        rewrite H. iFrame.
-      + cbn. rewrite (_: b_r + z + 1 = b_r + (z + 1)%nat)%Z; [|lia].
-        iFrame.
-      + iNext.
-        iIntros "(HPC & Hregion & Hrt & Hrt5 & Ha3 & Ha4 & Ha5 & Ha6 & Ha1 & Hrt2 & Hrt1 & Ha2 & Hrt4 & Hrt3)".
-        iApply "Hφ".
-        iFrame.
-        rewrite /region_addrs_zeroesL.
-        rewrite (finz_dist_S a_r e_r) //= (_: (a_r^+1)%a = a_r'); [| solve_addr].
-        iFrame.
-      + iPureIntro. intro.
-        rewrite andb_true_iff -Zle_is_le_bool -Zlt_is_lt_bool. solve_addr.
-      + iPureIntro. solve_addr.
-      + solve_addr.
-    - assert (Z.b2z (e_r - 1 <? b_r + z)%Z = 1%Z) as Heq0.
-      { rewrite /Z.b2z. destruct (e_r - 1 <? b_r + z)%Z eqn:HH; auto.
-        apply Z.ltb_nlt in HH. lia. }
-      rewrite Heq0.
-      assert (e_r <= a_r)%Z by solve_addr.
-      (* destruct (Z.le_dec a_r e_r). *)
-      rewrite finz_dist_0 //=.
-      destruct ws;[|by iApply bi.False_elim].
-      (* jnz *)
-      iDestruct "Hprog" as "[Hi Hprog]".
-      iApply (wp_bind (fill [SeqCtx])).
-      iApply (wp_jnz_success_jmp _ rt4 rt3 _ _ _ a2 _ _ _ (LInt 1%Z) with "[HPC Hi Hr_t3 Hr_t4]"); first apply decode_encode_instrLW_inv; eauto.
-      iFrame. iEpilogue "(HPC & Ha2 & Hr_t4 & Hr_t3)".
-      iApply "Hφ". iDestruct "Hprog" as "(Ha3 & Ha4 & Ha5 & Ha6 & _)".
-      rewrite /region_addrs_zeroesL finz_dist_0 //=. iFrame.
-      iSplitL "Hrt"; eauto.
-  Qed.
+  (*   rewrite {1}/salloc_instrs. *)
+  (*   focus_block_0 "Hprog" as "Hfetch" "Hcont". *)
+  (*   iApply fetch_spec; iFrameAutoSolve. *)
+  (*   iNext. iIntros "(HPC & Hfetch & Hr_t1 & Hr_t2 & Hr_t3 & Hpc_b & Ha_entry)". *)
+  (*   unfocus_block "Hfetch" "Hcont" as "Hprog". *)
 
-  Lemma mclear_spec (a : list Addr) (r : RegName)
-        (a_first a6' a_end : Addr) p b e p_r (b_r e_r a_r : Addr) a' v
-        w1 w2 w3 w4 w5 w6 ws φ :
-    contiguous_between a a_first a' →
-    (* We will assume that we are not trying to clear memory in a *)
-    r ≠ PC ∧ writeAllowed p_r = true →
-    (a !! 7 = Some a6' ∧ (a6' + 10)%a = Some a_end ∧ a !! 17 = Some a_end) →
+  (*   focus_block 1 "Hprog" as amid1 Hamid1 "Hprog" "Hcont". *)
+  (*   iGo "Hprog". (* PC is now at b_m *) *)
+  (*   (* we are now ready to use the salloc subroutine spec. For this we prepare the registers *) *)
+  (*   iDestruct (big_sepM_insert _ _ r_t3 with "[$Hregs $Hr_t3]") as "Hregs". *)
+  (*     by simplify_map_eq. *)
+  (*   iDestruct (big_sepM_insert _ _ r_t2 with "[$Hregs $Hr_t2]") as "Hregs". *)
+  (*     by simplify_map_eq. *)
+  (*   map_simpl "Hregs". *)
+  (*   iDestruct (big_sepM_insert _ _ r_t5 with "[$Hregs $Hr_t5]") as "Hregs". *)
+  (*     by simplify_map_eq. *)
+  (*   map_simpl "Hregs". *)
+  (*   iApply (wp_wand with "[- Hφfailed Hψ]"). *)
+  (*   iApply (simple_salloc_subroutine_spec with "[- $Hsalloc $Hna $Hregs $Hr_t0 $HPC $Hr_t1]"); auto. *)
+  (*   { set_solver+ Hrmap_dom. } *)
+  (*   iNext. *)
+  (*   rewrite updatePcPermL_cap_non_E; [| solve_pure]. *)
+  (*   iIntros "((Hna & Hregs) & Hr_t0 & HPC & Hbe) /=". *)
+  (*   iDestruct "Hbe" as (b e size' Hsize' Hbe) "(Hr_t1 & Hbe)". inversion Hsize'; subst size'. *)
+  (*   iDestruct (big_sepM_delete _ _ r_t3 with "Hregs") as "[Hr_t3 Hregs]". *)
+  (*     simplify_map_eq. eauto. *)
+  (*   iDestruct (big_sepM_delete _ _ r_t5 with "Hregs") as "[Hr_t5 Hregs]". *)
+  (*     simplify_map_eq. eauto. *)
+  (*   (* back our program, in the continuation of salloc *) *)
+  (*   iGo "Hprog". *)
+  (*   unfocus_block "Hprog" "Hcont" as "Hprog". *)
+  (*   (* continuation *) *)
+  (*   iApply "Hφ". changePCto (a_first ^+ length (salloc_instrs f_m size)%nat)%a. *)
+  (*   iFrame. iSplitL "Hr_t1 Hbe". *)
+  (*   { iExists _,_. iFrame. iPureIntro; eauto. } *)
+  (*   { iDestruct (big_sepM_insert _ _ r_t5 with "[$Hregs $Hr_t5]") as "Hregs". *)
+  (*       simplify_map_eq. reflexivity. *)
+  (*     iDestruct (big_sepM_insert _ _ r_t3 with "[$Hregs $Hr_t3]") as "Hregs". *)
+  (*     simplify_map_eq. reflexivity. *)
+  (*     iFrameMapSolve+ Hrmap_dom "Hregs". } *)
+  (*   { iIntros (w) "[Hφ|Hφ] /=". iApply "Hψ". iFrame. iSimplifyEq. eauto. } *)
+  (* Qed. *)
 
-    isCorrectPC_range p b e a_first a' →
+  (* (* salloc spec - alternative formulation *) *)
+  (* Lemma salloc_spec φ size cont pc_p pc_b pc_e v a_first *)
+  (*       b_link e_link a_link f_m a_entry sallocN b_m e_m EN rmap : *)
+  (*   ExecPCPerm pc_p → *)
+  (*   SubBounds pc_b pc_e a_first (a_first ^+ length (salloc_instrs f_m size))%a → *)
+  (*   withinBounds b_link e_link a_entry = true → *)
+  (*   (a_link + f_m)%a = Some a_entry → *)
+  (*   dom rmap = all_registers_s ∖ {[ PC; r_t0 ]} → *)
+  (*   ↑sallocN ⊆ EN → *)
+  (*   (size > 0)%Z → *)
 
-    (* We will also assume the region to clear is non empty *)
-    (b_r ≤ e_r)%Z →
-
-     (mclear a r v
-    ∗ ▷ PC ↦ᵣ LCap p b e a_first v
-    ∗ ▷ r ↦ᵣ LCap p_r b_r e_r a_r v
-    ∗ ▷ r_t4 ↦ᵣ w4
-    ∗ ▷ r_t1 ↦ᵣ w1
-    ∗ ▷ r_t2 ↦ᵣ w2
-    ∗ ▷ r_t3 ↦ᵣ w3
-    ∗ ▷ r_t5 ↦ᵣ w5
-    ∗ ▷ r_t6 ↦ᵣ w6
-    ∗ ▷ ([[ b_r , e_r ]] ↦ₐ{v} [[ ws ]])
-    ∗ ▷ (PC ↦ᵣ LCap p b e a' v
-            ∗ r_t1 ↦ᵣ LInt 0%Z
-            ∗ r_t2 ↦ᵣ LInt 0%Z
-            ∗ r_t3 ↦ᵣ LInt 0%Z
-            ∗ r_t4 ↦ᵣ LInt 0%Z
-            ∗ r_t5 ↦ᵣ LInt 0%Z
-            ∗ r_t6 ↦ᵣ LInt 0%Z
-            ∗ r ↦ᵣ LCap p_r b_r e_r a_r v
-            ∗ [[ b_r , e_r ]] ↦ₐ{v} [[region_addrs_zeroesL b_r e_r v]]
-            ∗ mclear a r v -∗
-            WP Seq (Instr Executable) {{ φ }})
-    ⊢ WP Seq (Instr Executable) {{ φ }})%I.
-  Proof.
-    iIntros (Hnext [Hne Hwa] Hjnz_off Hvpc Hle)
-            "(Hmclear & >HPC & >Hr & >Hr_t4 & >Hr_t1 & >Hr_t2 & >Hr_t3 & >Hr_t5 & >Hr_t6 & >Hregion & Hφ)".
-    iAssert (⌜((length a) =? (length (mclear_instrs r)) = true)%nat⌝)%I as %Hlen.
-    { destruct (((length a) =? (length (mclear_instrs r)))%nat) eqn:Hlen; auto.
-      rewrite /mclear Hlen. by iApply bi.False_elim. }
-    rewrite /mclear Hlen /mclear_instrs; simpl in Hlen. apply Nat.eqb_eq in Hlen.
-    destruct a as [| a1 a]; inversion Hlen; simpl.
-    move: (contiguous_between_cons_inv_first _ _ _ _ Hnext).
-    match goal with |- (?a = _) -> _ => intro; subst a end.
-    iPrologue "Hmclear".
-    iApply (wp_move_success_reg _ _ _ _ a_first _ _ _ r_t4 _ r with "[HPC Hr Hr_t4 Hi]");
-      first apply decode_encode_instrLW_inv; first iCorrectLPC a_first a'; eauto.
-    { iContiguous_next Hnext 0. }
-    iFrame. iEpilogue "(HPC & Ha_first & Hr_t4 & Hr)".
-    (* getb r_t1 r_t4 *)
-    iPrologue "Hprog".
-    iApply (wp_Get_success _ _ r_t1 r_t4 _ _ _ a0 with "[$HPC $Hi $Hr_t1 $Hr_t4]");
-      first eapply decode_encode_instrLW_inv; first eauto; first iCorrectLPC a_first a'; eauto.
-    { iContiguous_next Hnext 1. }
-    iFrame. iEpilogue "(HPC & Ha0 & Hr_t4 & Hr_t1)".
-    destruct (reg_eq_dec PC r_t4) as [Hcontr | _]; [inversion Hcontr|].
-    iCombine "Ha0 Ha_first" as "Hprog_done".
-    (* geta r_t2 r_t4 *)
-    iPrologue "Hprog".
-    iApply (wp_Get_success _ _ r_t2 r_t4 _ _ _ a1 with "[HPC Hi Hr_t2 Hr_t4]");
-      first eapply decode_encode_instrLW_inv; first eapply is_Get_GetA ; first iCorrectLPC a_first a'; auto.
-    { iContiguous_next Hnext 2. }
-    2: iFrame. auto. iEpilogue "(HPC & Ha1 & Hr_t4 & Hr_t2)".
-    destruct (reg_eq_dec PC r_t4) as [Hcontr | _]; [inversion Hcontr|].
-    iCombine "Ha1 Hprog_done" as "Hprog_done".
-    (* sub r_t2 r_t1 r_t2 *)
-    iPrologue "Hprog".
-    (* destruct b_r eqn:Hb_r. *)
-    iApply (wp_add_sub_lt_success_r_dst _ _ _ _ _ a2 _ _ _ r_t1 with "[HPC Hi Hr_t1 Hr_t2]"); try iFrame;
-      [ apply decode_encode_instrLW_inv | | |..]; eauto. 2: by iCorrectLPC a_first a'.
-    assert ((a2 + 1) = Some a3)%a as ->. { iContiguous_next Hnext 3. } by eauto.
-    iEpilogue "(HPC & Ha2 & Hr_t1 & Hr_t2)".
-    iCombine "Ha2 Hprog_done" as "Hprog_done".
-    (* lea r_t4 r_t2 *)
-    iPrologue "Hprog".
-    assert (a_r + (b_r - a_r) = b_r)%Z as Haddmin; first lia.
-    assert ((a_r + (b_r - a_r))%a = Some b_r) as Ha_rb_r by solve_addr.
-    iApply (wp_lea_success_reg _ _ _ _ a3 a4 _ _ r_t4 r_t2 p_r _ _ a_r _ (b_r - a_r) with "[HPC Hi Hr_t4 Hr_t2]");
-      first apply decode_encode_instrLW_inv; first iCorrectLPC a_first a'; eauto.
-    { iContiguous_next Hnext 4. }
-    { destruct p_r; inversion Hwa; auto. }
-    by iFrame. iEpilogue "(HPC & Ha3 & Hr_t2 & Hr_t4)".
-    iCombine "Ha3 Hprog_done" as "Hprog_done".
-    (* gete r_t2 r_t4 *)
-    iPrologue "Hprog".
-    iApply (wp_Get_success _ _ r_t5 r_t4 _ _ _ a4 with "[HPC Hi Hr_t5 Hr_t4]"); try iFrame;
-      first apply decode_encode_instrLW_inv; first eauto; first iCorrectLPC a_first a'; eauto.
-    { iContiguous_next Hnext 5. }
-    destruct (reg_eq_dec PC r_t4) as [Hcontr | _]; [inversion Hcontr|].
-    destruct (reg_eq_dec r_t4 r_t5) as [Hcontr | _]; [inversion Hcontr|].
-    iEpilogue "(HPC & Ha4 & Hr_t4 & Hr_t5)".
-    iCombine "Ha4 Hprog_done" as "Hprog_done".
-    (* sub r_t5 r_t5 1 *)
-    iPrologue "Hprog".
-    iApply (wp_add_sub_lt_success_dst_z with "[$HPC $Hi Hr_t5]");
-      [apply decode_encode_instrLW_inv| | |iCorrectLPC a_first a'|..]; eauto.
-    assert ((a5 + 1)%a = Some a6) as ->. { iContiguous_next Hnext 6. } eauto.
-    iEpilogue "(HPC & Ha5 & Hr_t5)".
-    iCombine "Ha5 Hprog_done" as "Hprog_done".
-    (* move r_t2 PC *)
-    iPrologue "Hprog".
-    iApply (wp_move_success_reg_fromPC _ _ _ _ a6 _ a7 _ r_t2 with "[HPC Hi Hr_t2]");
-      first apply decode_encode_instrLW_inv; first iCorrectLPC a_first a'; eauto.
-    { iContiguous_next Hnext 7. }
-    iFrame. iEpilogue "(HPC & Ha6 & Hr_t2)".
-    iCombine "Ha6 Hprog_done" as "Hprog_done".
-    (* lea r_t2 mclear_off_end *)
-    iPrologue "Hprog".
-    assert (p ≠ E) as Hpne.
-    { have: (isCorrectPC (WCap p b e a_first)).
-      { apply Hvpc. eapply contiguous_between_middle_bounds'; eauto. constructor. }
-      inversion 1; subst.
-      destruct H15 as [? | ? ]; subst; auto. }
-    iApply (wp_lea_success_z _ _ _ _ a7 a8 _ _ r_t2 p _ _ a6 _ 10 a_end with "[HPC Hi Hr_t2]");
-      first apply decode_encode_instrLW_inv; first iCorrectLPC a_first a'; auto.
-    { iContiguous_next Hnext 8. }
-    { destruct Hjnz_off as (Ha7' & Hmclear_off_end & Ha_end). simpl in Ha7'. congruence. }
-    iFrame. iEpilogue "(HPC & Ha7 & Hr_t2)".
-    iCombine "Ha7 Hprog_done" as "Hprog_done".
-    (* move r_t3 PC *)
-    iPrologue "Hprog".
-    iApply (wp_move_success_reg_fromPC _ _ _ _ a8 _ a9 _ r_t3 with "[HPC Hi Hr_t3]");
-      first apply decode_encode_instrLW_inv; first iCorrectLPC a_first a'; auto.
-    { iContiguous_next Hnext 9. }
-    iFrame. iEpilogue "(HPC & Ha8 & Hr_t3)".
-    iCombine "Ha8 Hprog_done" as "Hprog_done".
-    (* lea r_t3 mclear_off_iter *)
-    iPrologue "Hprog".
-    iApply (wp_lea_success_z _ _ _ _ a9 a10 _ _ r_t3 p _ _ a8 _ 2 a10 with "[HPC Hi Hr_t3]");
-      first apply decode_encode_instrLW_inv; first iCorrectLPC a_first a'; auto.
-    { iContiguous_next Hnext 10. }
-    { assert (2 = 1 + 1)%Z as ->; auto.
-      apply incr_addr_trans with a9. iContiguous_next Hnext 9.
-      iContiguous_next Hnext 10. }
-    iFrame. iEpilogue "(HPC & Ha9 & Hr_t3)".
-    iCombine "Ha9 Hprog_done" as "Hprog_done".
-    (* iter *)
-    clear H0 H1 H2 H3 H4 H5 H6 H7 H8 H9.
-    do 5 iPrologue_pre. clear H0 H1 H2 H3.
-    iDestruct "Hprog" as "[Hi1 Hprog]".
-    iDestruct "Hprog" as "[Hi2 Hprog]".
-    iDestruct "Hprog" as "[Hi3 Hprog]".
-    iDestruct "Hprog" as "[Hi4 Hprog]".
-    iDestruct "Hprog" as "[Hi5 Hprog]".
-    iDestruct "Hprog" as "[Hi6 Hprog]".
-    iApply (mclear_iter_spec a10 a11 a12 a13 a14 a15 b_r e_r b_r _ _
-                        0 p b e r_t4 r_t1 r_t5 r_t6 r_t2 r_t3 _ p_r
-              with "[-]"); auto.
-    - repeat apply conj; iCorrectLPC a_first a'.
-    - repeat split; solve [
-        iContiguous_next Hnext 11; auto
-      | iContiguous_next Hnext 12; auto
-      | iContiguous_next Hnext 13; auto
-      | iContiguous_next Hnext 14; auto
-      | iContiguous_next Hnext 15; auto ].
-    - (* rewrite Z.add_0_r. intros Hle. *)
-      rewrite /withinBounds. intro.
-      rewrite andb_true_iff Z.leb_le Z.ltb_lt. lia.
-    - apply addr_add_0.
-    - rewrite Z.add_0_r.
-      iFrame.
-      iSplitL "Hr_t6". iNext. iExists w6. iFrame.
-      iSplitR; auto.
-      iNext.
-      iIntros "(HPC & Hbe & Hr_t4 & Hr_t3 & Ha11 & Ha12 & Ha13 & Ha14 &
-      Ha9 & Hr_t5 & Hr_t1 & Ha10 & Hr_t2 & Hr_t6)".
-      iCombine "Ha9 Ha10 Ha11 Ha12 Ha13 Ha14 Hprog_done" as "Hprog_done".
-      iDestruct "Hr_t4" as (a_r0) "Hr_t4".
-      iDestruct "Hr_t1" as (z0) "Hr_t1".
-      iPrologue "Hprog".
-      assert (a16 = a_end)%a as Ha16.
-      { simpl in Hjnz_off.
-        destruct Hjnz_off as (Ha16 & Ha16' & Hend).
-        by inversion Hend.
-      }
-      destruct a as [| a17 a]; inversion Hlen.
-      iApply (wp_move_success_z _ _ _ _ a16 a17 _ _ r_t4 _ 0 with "[HPC Hi Hr_t4]");
-        first apply decode_encode_instrLW_inv;
-        first iCorrectLPC a_first a'; auto.
-      { iContiguous_next Hnext 17; auto. }
-      { rewrite Ha16. destruct p; iFrame. contradiction. }
-      iEpilogue "(HPC & Ha16 & Hr_t4)".
-      (* move r_t1 0 *)
-      iPrologue "Hprog".
-      iApply (wp_move_success_z _ _ _ _ a17 a18 _ _ r_t1 _ 0 with "[HPC Hi Hr_t1]");
-        first apply decode_encode_instrLW_inv;
-        first iCorrectLPC a_first a'; auto.
-      { iContiguous_next Hnext 18. }
-      iFrame. iEpilogue "(HPC & Ha17 & Hr_t1)".
-      (* move r_t2 0 *)
-      iPrologue "Hprog".
-      iApply (wp_move_success_z _ _ _ _ a18 a19 _ _ r_t2 _ 0 with "[HPC Hi Hr_t2]");
-        first apply decode_encode_instrLW_inv;
-        first iCorrectLPC a_first a'; auto.
-      { iContiguous_next Hnext 19. }
-      iFrame. iEpilogue "(HPC & Ha18 & Hr_t2)".
-      (* move r_t3 0 *)
-      iPrologue "Hprog".
-      iApply (wp_move_success_z _ _ _ _ a19 a20 _ _ r_t3 _ 0 with "[HPC Hi Hr_t3]");
-        first apply decode_encode_instrLW_inv;
-        first iCorrectLPC a_first a'; auto.
-      { iContiguous_next Hnext 20. }
-      iFrame. iEpilogue "(HPC & Ha19 & Hr_t3)".
-      (* move r_t5 0 *)
-      iPrologue "Hprog".
-      iApply (wp_move_success_z _ _ _ _ a20 a21 _ _ r_t5 _ 0 with "[HPC Hi Hr_t5]");
-        first apply decode_encode_instrLW_inv;
-        first iCorrectLPC a_first a'; auto.
-      { iContiguous_next Hnext 21. }
-      simplify_eq;  rewrite H6; iFrame.
-      iEpilogue "(HPC & Ha20 & Hr_t5)".
-      (* move r_t6 0 *)
-      iPrologue "Hprog".
-      iApply (wp_move_success_z _ _ _ _ a21 a' _ _ r_t6 _ 0 with "[HPC Hi Hr_t6]");
-        first apply decode_encode_instrLW_inv;
-        first iCorrectLPC a_first a'; auto.
-      { eapply contiguous_between_last. eapply Hnext. reflexivity. }
-      iFrame. iEpilogue "(HPC & Ha21 & Hr_t6)".
-      iApply "Hφ".
-      iDestruct "Hprog_done" as "(Ha_iter & Ha10 & Ha12 & Ha11 & Ha13 & Ha14 & Ha15 & Ha8 & Ha7
-      & Ha6 & Ha5 & Ha4 & Ha3 & Ha2 & Ha1 & Ha0 & Ha_first)".
-      iFrame.
-  Qed.
-
-
+  (*   (* salloc program and subroutine *) *)
+  (*   ▷ codefrag a_first v (salloc_instrs f_m size) *)
+  (*   ∗ na_inv logrel_nais sallocN (salloc_inv b_m e_m v) *)
+  (*   ∗ na_own logrel_nais EN *)
+  (*   (* we need to assume that the salloc capability is in the linking table at offset f_m *) *)
+  (*   ∗ ▷ (pc_b,v) ↦ₐ LCap RO b_link e_link a_link v *)
+  (*   ∗ ▷ (a_entry,v) ↦ₐ LCap E b_m e_m b_m v *)
+  (*   (* register state *) *)
+  (*   ∗ ▷ PC ↦ᵣ LCap pc_p pc_b pc_e a_first v *)
+  (*   ∗ ▷ r_t0 ↦ᵣ cont *)
+  (*   ∗ ▷ ([∗ map] r_i↦w_i ∈ rmap, r_i ↦ᵣ w_i) *)
+  (*   (* continuation *) *)
+  (*   ∗ ▷ (PC ↦ᵣ LCap pc_p pc_b pc_e (a_first ^+ length (salloc_instrs f_m size))%a v *)
+  (*        ∗ codefrag a_first v (salloc_instrs f_m size) *)
+  (*        ∗ (pc_b,v) ↦ₐ LCap RO b_link e_link a_link v *)
+  (*        ∗ (a_entry,v) ↦ₐ LCap E b_m e_m b_m v *)
+  (*        (* the newly allocated region *) *)
+  (*        ∗ (∃ (bs es : OType), *)
+  (*           ⌜(bs + size)%ot = Some es⌝ *)
+  (*           ∗ r_t1 ↦ᵣ LSealRange (true,true) bs es bs *)
+  (*           ∗ ([∗ list] o ∈ finz.seq_between bs es, can_alloc_pred o)) *)
+  (*        ∗ r_t0 ↦ᵣ cont *)
+  (*        ∗ na_own logrel_nais EN *)
+  (*        ∗ ([∗ map] r_i↦w_i ∈ (<[r_t2:=LInt 0%Z]> *)
+  (*                              (<[r_t3:=LInt 0%Z]> *)
+  (*                               (<[r_t4:=LInt 0%Z]> *)
+  (*                                (<[r_t5:=LInt 0%Z]> (delete r_t1 rmap))))), r_i ↦ᵣ w_i) *)
+  (*        (* the newly allocated region is fresh in the current world *) *)
+  (*        (* ∗ ⌜Forall (λ a, a ∉ dom (gset Addr) (std W)) (finz.seq_between b e)⌝ *) *)
+  (*        -∗ WP Seq (Instr Executable) {{ φ }}) *)
+  (*   ⊢ *)
+  (*     WP Seq (Instr Executable) {{ λ v, φ v ∨ ⌜v = FailedV⌝ }}. *)
+  (* Proof. *)
+  (*   iIntros (Hvpc Hcont Hwb Ha_entry Hrmap_dom HsallocN Hsize) *)
+  (*           "(>Hprog & #Hsalloc & Hna & >Hpc_b & >Ha_entry & >HPC & >Hr_t0 & >Hregs & Hφ)". *)
+  (*   iApply salloc_spec_alt; iFrameAutoSolve; eauto. iFrame. iFrame "Hsalloc". *)
+  (*   iSplitL. iNext. eauto. eauto. *)
+  (* Qed. *)
 
   (* -------------------------------------- REQPERM ----------------------------------- *)
   (* the following macro requires that a given registers contains a capability with a
      given (encoded) permission. If this is not the case, the macro goes to fail,
      otherwise it continues *)
 
+  (* ------------------------------- *)
   Definition reqperm_instrs r z :=
     encodeInstrsLW [
-    GetWType r_t1 r;
-    Sub r_t1 r_t1 (encodeWordType wt_cap);
-    Mov r_t2 PC;
-    Lea r_t2 11;
-    Jnz r_t2 r_t1; (* if is_int(r) then jmp LABEL*)
-    GetP r_t1 r;
-    Sub r_t1 r_t1 z;
-    Mov r_t2 PC;
-    Lea r_t2 6;
-    Jnz r_t2 r_t1;
-    Mov r_t2 PC;
-    Lea r_t2 4;
-    Jmp r_t2;
-    Fail;
-    Mov r_t1 0;
-    Mov r_t2 0].
+        GetWType r_t1 r;
+        Sub r_t1 r_t1 (encodeLWordType lwt_cap);
+        Mov r_t2 PC;
+        Lea r_t2 11;
+        Jnz r_t2 r_t1;
+        GetP r_t1 r;
+         Sub r_t1 r_t1 z
+        ; Mov r_t2 PC
+        ; Lea r_t2 6
+        ; Jnz r_t2 r_t1
+        ; Mov r_t2 PC
+        ; Lea r_t2 4
+        ; Jmp r_t2
+        ; Fail
+        ; Mov r_t1 0
+        ; Mov r_t2 0].
 
-  Definition reqperm r z a v : iProp Σ :=
-    ([∗ list] a_i;w_i ∈ a;(reqperm_instrs r z), (a_i, v) ↦ₐ w_i)%I.
+  Lemma reqperm_spec r perm w pc_p pc_b pc_e v a_first w1 w2 φ :
+    ExecPCPerm pc_p →
+    SubBounds pc_b pc_e a_first (a_first ^+ length (reqperm_instrs r (encodePerm perm)))%a →
 
-  Lemma reqperm_spec r perm a w pc_p pc_b pc_e v a_first a_last φ :
-    isCorrectPC_range pc_p pc_b pc_e a_first a_last ->
-    contiguous_between a a_first a_last ->
-
-      ▷ reqperm r (encodePerm perm) a v
+      ▷ codefrag a_first v (reqperm_instrs r (encodePerm perm))
     ∗ ▷ PC ↦ᵣ LCap pc_p pc_b pc_e a_first v
     ∗ ▷ r ↦ᵣ w
-    ∗ ▷ (∃ w, r_t1 ↦ᵣ w)
-    ∗ ▷ (∃ w, r_t2 ↦ᵣ w)
+    ∗ ▷ r_t1 ↦ᵣ w1
+    ∗ ▷ r_t2 ↦ᵣ w2
     ∗ ▷ (if isPermLWord w perm then
            ∃ b e a', ⌜w = LCap perm b e a' v⌝ ∧
-          (PC ↦ᵣ LCap pc_p pc_b pc_e a_last v ∗ reqperm r (encodePerm perm) a v ∗
+           (PC ↦ᵣ LCap pc_p pc_b pc_e (a_first ^+ length (reqperm_instrs r (encodePerm perm)))%a v
+            ∗ codefrag a_first v (reqperm_instrs r (encodePerm perm)) ∗
             r ↦ᵣ LCap perm b e a' v ∗ r_t1 ↦ᵣ LInt 0%Z ∗ r_t2 ↦ᵣ LInt 0%Z
             -∗ WP Seq (Instr Executable) {{ φ }})
         else φ FailedV)
     ⊢
       WP Seq (Instr Executable) {{ φ }}.
   Proof.
-    iIntros (Hvpc Hcont) "(>Hprog & >HPC & >Hr & >Hr_t1 & >Hr_t2 & Hcont)".
-    iDestruct (big_sepL2_length with "Hprog") as %Hlength. simpl in *.
-    iDestruct ("Hr_t1") as (w1) "Hr_t1".
-    iAssert (⌜r ≠ PC⌝)%I as %Hne.
-    { destruct (decide (r = PC)); auto; subst. iDestruct (regname_dupl_false with "HPC Hr") as %Hcontr. done. }
-
-    iPrologue "Hprog".
-    apply contiguous_between_cons_inv_first in Hcont as Heq. subst.
-    destruct a as [|a l];[done|].
-    iApply (wp_Get_success with "[$HPC $Hi $Hr $Hr_t1]")
-    ; [apply decode_encode_instrLW_inv|solve_pure|iCorrectLPC a_first a_last |iContiguous_next Hcont 0|auto..].
-
-    iEpilogue "(HPC & Hi & Hr & Hr_t1)". iRename "Hi" into "Hprog_done".
-
-    iPrologue "Hprog".
-    destruct l;[done|].
-    iApply (wp_add_sub_lt_success_dst_z with "[$HPC $Hi $Hr_t1]");
-      [apply decode_encode_instrLW_inv|auto|iContiguous_next Hcont 1|iCorrectLPC a_first a_last|..].
-    iEpilogue "(HPC & Hi & Hr_t1)". iCombine "Hi" "Hprog_done" as "Hprog_done".
-    iSimpl in "Hr_t1".
-
-    iPrologue "Hprog".
-    destruct l;[done|].
-    iDestruct "Hr_t2" as (w2) "Hr_t2".
-    iApply (wp_move_success_reg_fromPC with "[$HPC $Hi $Hr_t2]");
-      [apply decode_encode_instrLW_inv|iCorrectLPC a_first a_last|iContiguous_next Hcont 2|auto|..].
-    iEpilogue "(HPC & Hi & Hr_t2)"; iCombine "Hi" "Hprog_done" as "Hprog_done".
-
-    iPrologue "Hprog".
-    do 12 (destruct l;[done|]).
-    assert ((f + 11)%a = Some f10) as Hlea.
-    { apply (contiguous_between_incr_addr_middle _ _ _ 2 11 f f10) in Hcont; auto. }
-    assert (pc_p ≠ E) as HneE.
-    { apply isCorrectPC_range_perm in Hvpc as [Heq | Heq ]; subst; auto.
-      apply (contiguous_between_middle_bounds _ 0 a_first) in Hcont as [_ Hlt]; auto. }
-    iApply (wp_lea_success_z with "[$HPC $Hi $Hr_t2]");
-      [apply decode_encode_instrLW_inv|iCorrectLPC a_first a_last|iContiguous_next Hcont 3| exact |simpl;auto..].
-    iEpilogue "(HPC & Hi & Hr_t2)"; iCombine "Hi" "Hprog_done" as "Hprog_done".
-
-    destruct (is_log_cap w) eqn:Hcap ; cycle 1.
+    iIntros (Hvpc Hcont) "(>Hprog & >HPC & >Hr & >Hr_t1 & >Hr_t2 & Hφ)".
+    codefrag_facts "Hprog".
+    iGo "Hprog".
+    eapply getwtype_denote ; reflexivity .
+    do 3 iInstr "Hprog".
+    destruct (is_log_cap w) eqn:Hcap; cycle 1.
     {
       assert (isPermLWord w perm = false) as ->. {destruct_lword w; auto. inversion Hcap. }
 
       (* if w is not a capability we jump to the failure case *)
-      iPrologue "Hprog".
-      iApply (wp_jnz_success_jmp with "[$HPC $Hi $Hr_t2 $Hr_t1]");
-        [apply decode_encode_instrLW_inv|iCorrectLPC a_first a_last|..].
-      { intros Hcontr; clear -Hcap Hcontr.
+      iInstr "Hprog".
+      (* TODO maybe I could generalize this next sub-proof ? *)
+     { rewrite -/(encodeLWordType w).
+       intros Hcontr; clear -Hcap Hcontr.
         destruct w; [| (destruct sb; [by simpl in Hcap|]) |]
-        ; unfold wt_cap in Hcontr
+        ; unfold lwt_cap in Hcontr
         ; injection Hcontr
         ; clear Hcontr; intro Hcontr
         ; apply Zminus_eq in Hcontr
         ; match goal with
-          | H: encodeWordType ?x = encodeWordType ?y |- _ =>
-              pose proof (encodeWordType_correct x y) as Hcontr2 ; cbn in Hcontr2
+          | H: encodeLWordType ?x = encodeLWordType ?y |- _ =>
+              pose proof (encodeLWordType_correct x y) as Hcontr2 ; cbn in Hcontr2
           end
         ; auto.
       }
-      iEpilogue "(HPC & Hi & Hr_t2 & Hr_t1)"; iCombine "Hi" "Hprog_done" as "Hprog_done".
-      do 8 (iDestruct "Hprog" as "[Hi Hprog]"; iCombine "Hi" "Hprog_done" as "Hprog_done").
-      (* fail *)
-      iPrologue "Hprog".
-      assert (updatePcPermL (LCap pc_p pc_b pc_e f10 v) = (LCap pc_p pc_b pc_e f10 v)) as ->.
-      { destruct pc_p; auto. congruence. }
-      iApply (wp_fail with "[$HPC $Hi]");
-        [apply decode_encode_instrLW_inv|iCorrectLPC a_first a_last|].
-      iEpilogue "(HPC & Hi)". iApply wp_value. iApply "Hcont".
-    }
-
+      rewrite -/(updatePcPermL (LCap _ _ _ _ _)). rewrite updatePcPermL_cap_non_E;[|inv Hvpc;auto].
+      iGo "Hprog".
+      by wp_end. }
+    {
     (* now we know that w is a capability *)
     assert (∃ p b e a v, w = LCap p b e a v)  as (pc & bc & ec & ac & vc & ->).
     {destruct_lword w ; inversion Hcap. eexists _,_,_,_,_; eauto. }
-    rewrite (_: (encodeWordType (lword_get_word (LCap pc bc ec ac vc)) - encodeWordType wt_cap)%Z = 0%Z); cycle 1.
-    { rewrite (_ : (encodeWordType (lword_get_word (LCap pc bc ec ac vc)))%Z = (encodeWordType wt_cap)%Z)
-      ; first lia. apply encodeWordType_correct_cap.
-    }
-    iPrologue "Hprog".
-    iApply (wp_jnz_success_next with "[$HPC $Hi $Hr_t2 $Hr_t1]");
-      [apply decode_encode_instrLW_inv|iCorrectLPC a_first a_last|iContiguous_next Hcont 4|..].
-    iEpilogue "(HPC & Hi & Hr_t2 & Hr_t1)"; iCombine "Hi" "Hprog_done" as "Hprog_done".
-
-    iPrologue "Hprog".
-    iApply (wp_Get_success with "[$HPC $Hi $Hr $Hr_t1]");
-      [apply decode_encode_instrLW_inv|auto|iCorrectLPC a_first a_last|iContiguous_next Hcont 5|auto..].
-    iEpilogue "(HPC & Hi & Hr & Hr_t1)". iCombine "Hi" "Hprog_done" as "Hprog_done".
-
-    (* sub r_t1 r_t1 (encodeLoc Global) *)
-    iPrologue "Hprog".
-    iApply (wp_add_sub_lt_success_dst_z with "[$HPC $Hi $Hr_t1]");
-      [apply decode_encode_instrLW_inv|auto|iContiguous_next Hcont 6|iCorrectLPC a_first a_last|..].
-    iEpilogue "(HPC & Hi & Hr_t1)". iCombine "Hi" "Hprog_done" as "Hprog_done".
-    iSimpl in "Hr_t1".
-
-    (* move r_t2 PC *)
-    iPrologue "Hprog".
-    iApply (wp_move_success_reg_fromPC with "[$HPC $Hi $Hr_t2]");
-      [apply decode_encode_instrLW_inv|iCorrectLPC a_first a_last|iContiguous_next Hcont 7|auto|..].
-    iEpilogue "(HPC & Hi & Hr_t2)"; iCombine "Hi" "Hprog_done" as "Hprog_done".
-
-    (* lea r_t2 6 *)
-    assert ((f4 + 6)%a = Some f10) as Hlea'.
-    { apply (contiguous_between_incr_addr_middle _ _ _ 7 6 f4 f10) in Hcont; auto. }
-    assert (pc_p ≠ E) as HneE'.
-    { apply isCorrectPC_range_perm in Hvpc as [Heq | Heq ]; subst; auto.
-      apply (contiguous_between_middle_bounds _ 0 a_first) in Hcont as [_ Hlt]; auto. }
-    iPrologue "Hprog".
-    iApply (wp_lea_success_z with "[$HPC $Hi $Hr_t2]");
-      [apply decode_encode_instrLW_inv|iCorrectLPC a_first a_last|iContiguous_next Hcont 8|apply Hlea'|auto..].
-    iEpilogue "(HPC & Hi & Hr_t2)"; iCombine "Hi" "Hprog_done" as "Hprog_done".
-    destruct (decide (encodePerm pc - encodePerm perm = 0))%Z as [e0|e0].
-    - (* p is perm *)
-      rewrite e0. assert (pc = perm);[apply encodePerm_inj;lia|subst].
-      iSimpl in "Hcont". rewrite isPerm_refl. iDestruct "Hcont" as (b0 e1 a' Heq) "Hφ". inversion Heq; subst.
-      iPrologue "Hprog".
-      iApply (wp_jnz_success_next with "[$HPC $Hi $Hr_t2 $Hr_t1]");
-        [apply decode_encode_instrLW_inv|iCorrectLPC a_first a_last|iContiguous_next Hcont 9|..].
-      iEpilogue "(HPC & Hi & Hr_t2 & Hr_t1)";iCombine "Hi" "Hprog_done" as "Hprog_done".
-      (* move_r r_t2 PC *)
-      iPrologue "Hprog".
-      iApply (wp_move_success_reg_fromPC with "[$HPC $Hi $Hr_t2]");
-        [apply decode_encode_instrLW_inv|iCorrectLPC a_first a_last|iContiguous_next Hcont 10|auto|..].
-      iEpilogue "(HPC & Hi & Hr_t2)"; iCombine "Hi" "Hprog_done" as "Hprog_done".
-      (* lea r_t2 3 *)
-      assert ((f7 + 4)%a = Some f11) as Hlea''.
-      { apply (contiguous_between_incr_addr_middle _ _ _ 10 4 f7 f11) in Hcont; auto. }
-      iPrologue "Hprog".
-      iApply (wp_lea_success_z with "[$HPC $Hi $Hr_t2]");
-        [apply decode_encode_instrLW_inv|iCorrectLPC a_first a_last|iContiguous_next Hcont 11|apply Hlea''|auto..].
-      iEpilogue "(HPC & Hi & Hr_t2)"; iCombine "Hi" "Hprog_done" as "Hprog_done".
-      (* jmp r_t2 *)
-      iPrologue "Hprog".
-      iApply (wp_jmp_success with "[$HPC $Hi $Hr_t2]");
-        [apply decode_encode_instrLW_inv|iCorrectLPC a_first a_last|..].
-      iEpilogue "(HPC & Hi & Hr_t2)"; iCombine "Hi" "Hprog_done" as "Hprog_done".
-      assert (updatePcPermL (LCap pc_p pc_b pc_e f11 v) = (LCap pc_p pc_b pc_e f11 v)) as ->.
-      { destruct pc_p; auto. congruence. }
-      iDestruct "Hprog" as "[Hi Hprog]". iCombine "Hi" "Hprog_done" as "Hprog_done".
-      (* move r_t1 0 *)
-      iPrologue "Hprog".
-      iApply (wp_move_success_z with "[$HPC $Hi $Hr_t1]");
-        [apply decode_encode_instrLW_inv|iCorrectLPC a_first a_last|iContiguous_next Hcont 14|auto|..].
-      iEpilogue "(HPC & Hi & Hr_t1)"; iCombine "Hi" "Hprog_done" as "Hprog_done".
-      (* move r_t2 0 *)
-      destruct l; [|done].
-      iPrologue "Hprog".
-      apply contiguous_between_last with (ai:=f12) in Hcont as Hnext;[|auto].
-      iApply (wp_move_success_z with "[$HPC $Hi $Hr_t2]");
-        [apply decode_encode_instrLW_inv|iCorrectLPC a_first a_last|apply Hnext|auto|..].
-      iEpilogue "(HPC & Hi & Hr_t2)"; iCombine "Hi" "Hprog_done" as "Hprog_done".
-      iApply "Hφ". iFrame "HPC Hr Hr_t1 Hr_t2".
-      do 15 (iDestruct "Hprog_done" as "[Hi Hprog_done]"; iFrame "Hi").
-      iFrame.
-    - assert (pc ≠ perm) as HneP.
-      { intros Hcontr. subst. lia. }
-      iSimpl in "Hcont". rewrite isPerm_ne;[|auto].
-      (* jnz r_t2 r_t1 *)
-      iPrologue "Hprog".
-      iApply (wp_jnz_success_jmp with "[$HPC $Hi $Hr_t2 $Hr_t1]");
-        [apply decode_encode_instrLW_inv|iCorrectLPC a_first a_last|..].
-      { intros Hcontr. inversion Hcontr. done. }
-      iEpilogue "(HPC & Hi & Hr_t2 & Hr_t1)"; iCombine "Hi" "Hprog_done" as "Hprog_done".
-      do 3 (iDestruct "Hprog" as "[Hi Hprog]"; iCombine "Hi" "Hprog_done" as "Hprog_done").
-      (* fail *)
-      iPrologue "Hprog".
-      assert (updatePcPermL (LCap pc_p pc_b pc_e f10 v) = (LCap pc_p pc_b pc_e f10 v)) as ->.
-      { destruct pc_p; auto. congruence. }
-      iApply (wp_fail with "[$HPC $Hi]");
-        [apply decode_encode_instrLW_inv|iCorrectLPC a_first a_last|].
-      iEpilogue "(HPC & Hi)". iApply wp_value. iApply "Hcont".
+    rewrite -/(encodeLWordType _).
+    simpl_encodeLWordType; rewrite Z.sub_diag.
+    do 5 iInstr "Hprog".
+    destruct (isPermLWord (LCap pc bc ec ac vc) perm) eqn:Hperm.
+    {
+      iInstr_lookup "Hprog" as "Hi" "Hcont".
+      wp_instr.
+      assert (encodePerm pc - encodePerm perm = 0)%Z as ->.
+      { inversion Hperm as [Hp]. apply bool_decide_eq_true_1 in Hp as ->. lia. }
+      iApply (wp_jnz_success_next with "[$HPC $Hi $Hr_t2 $Hr_t1]");iFrameAutoSolve.
+      iNext. iIntros "(HPC & Hi & Hr_t2 & Hr_t1)". wp_pure.
+      iDestruct ("Hcont" with "Hi") as "Hprog".
+      iGo "Hprog".
+      rewrite -/(updatePcPermL (LCap _ _ _ _ _)).
+      rewrite updatePcPermL_cap_non_E;[|inv Hvpc;auto].
+      iGo "Hprog".
+      iDestruct "Hφ" as (b' e' a' Heq) "Hφ". inv Heq.
+      iApply "Hφ"; iFrame. }
+    {
+      iGo "Hprog".
+      inversion Hperm as [Hp]. apply bool_decide_eq_false_1 in Hp. intros Hcontr; inversion Hcontr as [Heq].
+      apply Zminus_eq,encodePerm_inj in Heq. subst pc. done.
+      rewrite -/(updatePcPermL (LCap _ _ _ _ _)%a).
+      rewrite updatePcPermL_cap_non_E;[|inv Hvpc;auto].
+      iGo "Hprog".
+      iApply wp_value. iFrame. } }
   Qed.
 
   (* --------------------------------------- REQSIZE ----------------------------------- *)
   (* This macro checks that the capability in r covers a memory range of size
-     (i.e. e-b) greater than [minsize]. *)
+     (i.e. e-b) exactly equal to [minsize]. *)
 
-  Definition reqsize_instrs r (minsize: Z) :=
-    encodeInstrsLW [
-        GetB r_t1 r;
-        GetE r_t2 r;
-        Sub r_t1 r_t2 r_t1;
-        Lt r_t1 minsize r_t1;
-        Mov r_t2 PC;
-        Lea r_t2 4;
-        Jnz r_t2 r_t1;
-        Fail].
+  Definition reqsize_exact_instrs r (exsize : Z) :=
+    encodeInstrsLW
+      [ GetB r_t1 r ;
+      GetE r_t2 r;
+      Sub r_t1 r_t2 r_t1;
+      Sub r_t1 r_t1 exsize;
+      Mov r_t2 PC;
+      Lea r_t2 6;
+      Jnz r_t2 r_t1;
+      Mov r_t2 PC;
+      Lea r_t2 4;
+      Jmp r_t2;
+      Fail].
 
-  Definition reqsize r minsize a v : iProp Σ :=
-    ([∗ list] a_i;w_i ∈ a;(reqsize_instrs r minsize), (a_i,v) ↦ₐ w_i)%I.
+  Lemma reqsize_spec r minsize pc_p pc_b pc_e v a_first r_p r_b r_e r_a w1 w2 φ :
+    ExecPCPerm pc_p →
+    SubBounds pc_b pc_e a_first (a_first ^+ length (reqsize_exact_instrs r minsize))%a →
 
-  Lemma reqsize_spec r minsize a pc_p pc_b pc_e v a_first a_last r_p r_b r_e r_a w1 w2 φ :
-    isCorrectPC_range pc_p pc_b pc_e a_first a_last →
-    contiguous_between a a_first a_last →
-
-      ▷ reqsize r minsize a v
+      ▷ codefrag a_first v (reqsize_exact_instrs r minsize)
     ∗ ▷ PC ↦ᵣ LCap pc_p pc_b pc_e a_first v
     ∗ ▷ r ↦ᵣ LCap r_p r_b r_e r_a v
     ∗ ▷ r_t1 ↦ᵣ w1
     ∗ ▷ r_t2 ↦ᵣ w2
-    ∗ ▷ (if (minsize <? (r_e - r_b)%a)%Z then
+    ∗ ▷ (if (minsize =? (r_e - r_b)%a)%Z then
            (∃ w1 w2,
-            reqsize r minsize a v
-            ∗ PC ↦ᵣ LCap pc_p pc_b pc_e a_last v
+            codefrag a_first v (reqsize_exact_instrs r minsize)
+            ∗ PC ↦ᵣ LCap pc_p pc_b pc_e (a_first ^+ length (reqsize_exact_instrs r minsize))%a v
             ∗ r ↦ᵣ LCap r_p r_b r_e r_a v
             ∗ r_t1 ↦ᵣ w1
             ∗ r_t2 ↦ᵣ w2)
            -∗ WP Seq (Instr Executable) {{ φ }}
         else φ FailedV)
     ⊢
-    WP Seq (Instr Executable) {{ φ }}.
+      WP Seq (Instr Executable) {{ φ }}.
   Proof.
-    iIntros (Hvpc Hcont) "(>Hprog & >HPC & >Hr & >Hr1 & >Hr2 & Hcont)".
-    iDestruct (big_sepL2_length with "Hprog") as %Hlength. simpl in *.
-    iAssert (⌜r ≠ PC⌝)%I as %Hne.
-    { iIntros (->). iApply (regname_dupl_false with "HPC Hr"). }
-    destruct a as [| a l];[done|].
-    pose proof (contiguous_between_cons_inv_first _ _ _ _ Hcont) as ->.
-    assert (pc_p ≠ E).
-    { eapply isCorrectPC_range_perm_non_E; eauto.
-      generalize (contiguous_between_length _ _ _ Hcont). rewrite Hlength /=.
-      clear; solve_addr. }
-    (* getb r_t1 r *)
-    destruct l as [| ? l];[done|].
-    iPrologue "Hprog".
-    iApply (wp_Get_success with "[$HPC $Hi $Hr $Hr1]");
-      [apply decode_encode_instrLW_inv|auto|iCorrectLPC a_first a_last|iContiguous_next Hcont 0|auto..];
-      simpl.
-    iEpilogue "(HPC & Hi & Hr & Hr1)". iRename "Hi" into "Hprog_done".
-    (* gete r_t2 r *)
-    destruct l as [| ? l];[done|].
-    iPrologue "Hprog".
-    iApply (wp_Get_success with "[$HPC $Hi $Hr $Hr2]");
-      [apply decode_encode_instrLW_inv|auto|iCorrectLPC a_first a_last|iContiguous_next Hcont 1|auto..];
-      simpl.
-    iEpilogue "(HPC & Hi & Hr & Hr2)". iCombine "Hi" "Hprog_done" as "Hprog_done".
-    (* sub_r_r r_t1 r_t2 r_t1 *)
-    destruct l as [| ? l];[done|].
-    iPrologue "Hprog".
-    iApply (wp_add_sub_lt_success_r_dst with "[$HPC $Hi $Hr2 $Hr1]");
-      [apply decode_encode_instrLW_inv|done|iContiguous_next Hcont 2|iCorrectLPC a_first a_last|..];
-      simpl.
-    iEpilogue "(HPC & Hi & Hr2 & Hr1)". iCombine "Hi" "Hprog_done" as "Hprog_done".
-    (* lt_z_r r_t1 minsize r_t1 *)
-    destruct l as [| ? l];[done|].
-    iPrologue "Hprog".
-    iApply (wp_add_sub_lt_success_z_dst with "[$HPC $Hi $Hr1]");
-      [apply decode_encode_instrLW_inv|done|iContiguous_next Hcont 3|iCorrectLPC a_first a_last|..];
-      simpl.
-    iEpilogue "(HPC & Hi & Hr1)". iCombine "Hi" "Hprog_done" as "Hprog_done".
-    (* move_r r_t2 PC *)
-    destruct l as [| ? l];[done|].
-    iPrologue "Hprog".
-    iApply (wp_move_success_reg_fromPC with "[$HPC $Hi $Hr2]");
-      [apply decode_encode_instrLW_inv|iCorrectLPC a_first a_last|iContiguous_next Hcont 4|auto..].
-    iEpilogue "(HPC & Hi & Hr2)". iCombine "Hi" "Hprog_done" as "Hprog_done".
-    (* lea_z r_t2 4 *)
-    destruct l as [| ? l];[done|].
-    iPrologue "Hprog".
-    iApply (wp_lea_success_z with "[$HPC $Hi $Hr2]");
-      [apply decode_encode_instrLW_inv|iCorrectLPC a_first a_last|iContiguous_next Hcont 5|try done..].
-    { change 4%Z with (Z.of_nat (4%nat)).
-      (* FIXME: a bit annoying to have to specify the index manually *)
-      eapply (contiguous_between_middle_to_end _ _ _ 4); eauto. }
-    iEpilogue "(HPC & Hi & Hr2)". iCombine "Hi" "Hprog_done" as "Hprog_done".
-    (* jnz r_t2 r_t1 *)
-    destruct l as [| ? l];[done|].
-    iPrologue "Hprog".
-    destruct (minsize <? r_e - r_b)%Z eqn:Htest; simpl.
-    { iApply (wp_jnz_success_jmp with "[$HPC $Hr2 $Hr1 $Hi]");
-        [apply decode_encode_instrLW_inv|iCorrectLPC a_first a_last|done|..].
-      iEpilogue "(HPC & Hi & Hr2 & Hr1)". iApply "Hcont". iExists _,_.
-      rewrite updatePcPermL_cap_non_E //. iFrame.
-      iDestruct "Hprog_done" as "(?&?&?&?&?&?)". iFrame. }
-    { iApply (wp_jnz_success_next with "[$HPC $Hr2 $Hr1 $Hi]");
-        [apply decode_encode_instrLW_inv|iCorrectLPC a_first a_last|iContiguous_next Hcont 6|..].
-      iEpilogue "(HPC & Hi & Hr2 & Hr1)". iCombine "Hi" "Hprog_done" as "Hprog_done".
-      (* fail_end *)
-      iPrologue "Hprog".
-      iApply (wp_fail with "[$HPC $Hi]");
-        [apply decode_encode_instrLW_inv|iCorrectLPC a_first a_last|..].
-      iEpilogue "(HPC & Hi)". iApply wp_value. iApply "Hcont". }
+    iIntros (Hvpc Hcont) "(>Hprog & >HPC & >Hr & >Hr_t1 & >Hr_t2 & Hφ)".
+    codefrag_facts "Hprog".
+    do 6 iInstr "Hprog".
+
+    destruct (minsize =? r_e - r_b)%Z eqn:Hsize.
+    { iInstr_lookup "Hprog" as "Hi" "Hcont".
+      wp_instr.
+      assert (r_e - r_b - minsize = 0)%Z as ->.
+      { solve_addr. }
+      iApply (wp_jnz_success_next with "[$HPC $Hi $Hr_t2 $Hr_t1]");iFrameAutoSolve.
+      iNext. iIntros "(HPC & Hi & Hr_t2 & Hr_t1)". wp_pure.
+      iDestruct ("Hcont" with "Hi") as "Hprog".
+      iGo "Hprog".
+      rewrite -/(updatePcPermL (LCap pc_p pc_b pc_e (a_first ^+ 11)%a v)).
+      rewrite updatePcPermL_cap_non_E;[|by inv Hvpc].
+      iApply "Hφ". iExists _,_. iFrame. }
+    { iGo "Hprog". intros Hcontr. inv Hcontr. solve_addr.
+      rewrite -/(updatePcPermL ((LWSealable (LSCap pc_p pc_b pc_e (a_first ^+ 10)%a v)))).
+      rewrite updatePcPermL_cap_non_E;[|by inv Hvpc].
+      iGo "Hprog". iApply wp_value. iFrame. }
   Qed.
 
-  (* ---------------------------------------- CRTCLS ------------------------------------ *)
-  (* The following macro creates a closure with one variable. A more general create closure would
-     allow for more than one variable in the closure, but this is so far not necessary for our
-     examples. The closure allocates a new region with a capability to the closure code, the closure
-     variable, and the closure activation *)
+  (* -------------------------------------- RCLEAR ----------------------------------- *)
+  (* the following macro clears registers in r. a denotes the list of addresses
+     containing the instructions for the clear: |a| = |r| *)
+  Definition rclear_instrs (r : list RegName) :=
+    encodeInstrsLW (map (λ r_i, Mov r_i 0) r).
+
+  Lemma rclear_instrs_cons rr r: rclear_instrs (rr :: r) = encodeInstrWL (Mov rr 0) :: rclear_instrs r.
+  Proof. reflexivity. Qed.
+
+  Lemma rclear_spec (r: list RegName) (rmap : gmap RegName LWord) pc_p pc_b pc_e v a_first φ :
+    PC ∉ r →
+    r ≠ [] →
+    ExecPCPerm pc_p →
+    SubBounds pc_b pc_e a_first (a_first ^+ length (rclear_instrs r))%a →
+    list_to_set r = dom rmap →
+
+      ▷ ([∗ map] r_i↦w_i ∈ rmap, r_i ↦ᵣ w_i)
+    ∗ ▷ PC ↦ᵣ LCap pc_p pc_b pc_e a_first v
+    ∗ ▷ codefrag a_first v (rclear_instrs r)
+    ∗ ▷ (PC ↦ᵣ LCap pc_p pc_b pc_e (a_first ^+ length (rclear_instrs r))%a v
+            ∗ ([∗ map] r_i↦_ ∈ rmap, r_i ↦ᵣ LInt 0%Z)
+            ∗ codefrag a_first v (rclear_instrs r)
+            -∗ WP Seq (Instr Executable) {{ φ }})
+    ⊢ WP Seq (Instr Executable) {{ φ }}.
+  Proof.
+    iIntros (Hne Hnnil Hepc Hbounds Hrdom) "(>Hreg & >HPC & >Hrclear & Hφ)".
+    iRevert (Hbounds Hrdom).
+    iInduction (r) as [| r0 r'] "IH" forall (rmap a_first).
+    { congruence. }
+
+    iIntros (? Hrdom). cbn [list_to_set] in Hrdom.
+    assert (is_Some (rmap !! r0)) as [r0v Hr0].
+    { apply elem_of_dom. rewrite -Hrdom. set_solver. }
+    iDestruct (big_sepM_delete _ _ r0 with "Hreg") as "[Hr0 Hreg]". by eauto.
+    codefrag_facts "Hrclear".
+    iInstr "Hrclear". transitivity (Some (a_first ^+ 1)%a); auto. solve_addr.
+    destruct (decide (r' = [])).
+    { subst r'. iApply "Hφ". iFrame. iApply (big_sepM_delete _ _ r0); eauto. iFrame.
+      rewrite (_: delete r0 rmap = ∅) //. apply dom_empty_inv_L.
+      rewrite dom_delete_L -Hrdom. set_solver. }
+
+    iAssert (codefrag (a_first ^+ 1)%a v (rclear_instrs r') ∗
+             (codefrag (a_first ^+ 1)%a v (rclear_instrs r') -∗ codefrag a_first v (rclear_instrs (r0 :: r'))))%I
+    with "[Hrclear]" as "[Hrclear Hcont]".
+    { cbn. unfold codefrag. rewrite (region_mapsto_cons _ (a_first ^+ 1)%a). 2,3: solve_addr.
+      iDestruct "Hrclear" as "[? Hr]".
+      rewrite (_: ((a_first ^+ 1) ^+ (length (rclear_instrs r')))%a =
+                    (a_first ^+ (S (length (rclear_instrs r'))))%a). 2: solve_addr.
+      iFrame. eauto. }
+
+    match goal with H : SubBounds _ _ _ _ |- _ =>
+      rewrite (_: (a_first ^+ (length (rclear_instrs (r0 :: r'))))%a =
+                  ((a_first ^+ 1)%a ^+ length (rclear_instrs r'))%a) in H |- *
+    end.
+    2: unfold rclear_instrs; cbn; solve_addr.
+
+    destruct (decide (r0 ∈ r')).
+    { iDestruct (big_sepM_insert _ _ r0 with "[Hr0 $Hreg]") as "Hreg".
+      by rewrite lookup_delete//. by iFrame.
+      iApply ("IH" with "[] [] Hreg HPC Hrclear [Hφ Hcont]"); eauto.
+      { iPureIntro. set_solver. }
+      { iNext. iIntros "(? & Hreg & Hcode)". iApply "Hφ".
+        iFrame. iDestruct ("Hcont" with "Hcode") as "Hcode". iFrame.
+        iDestruct (big_sepM_insert with "Hreg") as "[? ?]". by rewrite lookup_delete//.
+        iApply (big_sepM_delete _ _ r0). done. iFrame. }
+      { iPureIntro. solve_pure_addr. }
+      { rewrite insert_delete_insert. iPureIntro. set_solver. } }
+    { iApply ("IH" with "[] [] Hreg HPC Hrclear [Hφ Hcont Hr0]"); eauto.
+      { iPureIntro. set_solver. }
+      { iNext. iIntros "(? & Hreg & Hcode)". iApply "Hφ".
+        iFrame. iDestruct ("Hcont" with "Hcode") as "Hcode". iFrame.
+        iApply (big_sepM_delete _ _ r0). done. iFrame. }
+      { iPureIntro. solve_pure_addr. }
+      {  iPureIntro. set_solver. } }
+  Qed.
+
+  (* --------------------------------------------------------------------------------- *)
+  (* ------------------------------------- CRTCLS ------------------------------------ *)
+  (* --------------------------------------------------------------------------------- *)
 
   (* encodings of closure activation code *)
-  Definition v1 := encodeInstr (Mov r_t1 (inr PC)).
-  Definition v2 := encodeInstr (Lea r_t1 (inl 7%Z)).
-  Definition v3 := encodeInstr (Load r_env r_t1).
-  Definition v4 := encodeInstr (Lea r_t1 (inl (-1)%Z)).
-  Definition v5 := encodeInstr (Load r_t1 r_t1).
-  Definition v6 := encodeInstr (Jmp r_t1).
+  (* CHANGE: the following code is changed to use r_t20 as a temp register rather than r_t1 *)
+  (* TODO: use this convention across more examples, with a fixed choice of param registers and temp registers *)
+  Definition v1 := encodeInstr (Mov r_t20 (inr PC)).
+  Definition v2 := encodeInstr (Lea r_t20 (inl 7%Z)).
+  Definition v3 := encodeInstr (Load r_env r_t20).
+  Definition v4 := encodeInstr (Lea r_t20 (inl (-1)%Z)).
+  Definition v5 := encodeInstr (Load r_t20 r_t20).
+  Definition v6 := encodeInstr (Jmp r_t20).
 
+  Definition activation_code : list LWord :=
+    encodeInstrsLW [ Mov r_t20 PC ; Lea r_t20 7 ; Load r_env r_t20 ; Lea r_t20 (-1)%Z ; Load r_t20 r_t20 ; Jmp r_t20].
   Definition activation_instrs wcode wenv : list LWord :=
-    [ LInt v1; LInt v2; LInt v3; LInt v4; LInt v5; LInt v6; wcode; wenv ].
+    activation_code ++ [ wcode; wenv ].
 
-  (* scrtcls: "static" crtcls. Requires a capability for the memory region where to write
-     the activation record.
+  Definition scrtcls_instrs (rcode rdata: RegName) :=
+    encodeInstrsLW [ Store r_t1 v1
+                  ; Lea r_t1 1
+                  ; Store r_t1 v2
+                  ; Lea r_t1 1
+                  ; Store r_t1 v3
+                  ; Lea r_t1 1
+                  ; Store r_t1 v4
+                  ; Lea r_t1 1
+                  ; Store r_t1 v5
+                  ; Lea r_t1 1
+                  ; Store r_t1 v6
+                  ; Lea r_t1 1
+                  ; Store r_t1 rcode
+                  ; Mov rcode 0
+                  ; Lea r_t1 1
+                  ; Store r_t1 rdata
+                  ; Mov rdata 0
+                  ; Lea r_t1 (-7)%Z
+                  ; Restrict r_t1 e
+                  ].
 
-     It assumes the pointer to the region for the activation record is in r_t1, the
-     code pointer is in register rcode, and the data pointer in rdata.
-  *)
-  Definition scrtcls_instrs (rcode rdata : RegName) :=
-    encodeInstrsLW [
-        Store r_t1 v1;
-        Lea r_t1 1;
-        Store r_t1 v2;
-        Lea r_t1 1;
-        Store r_t1 v3;
-        Lea r_t1 1;
-        Store r_t1 v4;
-        Lea r_t1 1;
-        Store r_t1 v5;
-        Lea r_t1 1;
-        Store r_t1 v6;
-        Lea r_t1 1;
-        Store r_t1 rcode;
-        Mov rcode 0;
-        Lea r_t1 1;
-        Store r_t1 rdata;
-        Mov rdata 0;
-        Lea r_t1 (-7)%Z;
-        Restrict r_t1 e].
-
-  Definition scrtcls rcode rdata a v : iProp Σ :=
-    ([∗ list] a_i;w_i ∈ a;(scrtcls_instrs rcode rdata), (a_i,v) ↦ₐ w_i)%I.
-
-  (* crtcls: calls malloc to allocate memory for the activation record, then scrtcls. *)
-  (* f_m denotes the offset to the malloc capability in the lookup table *)
-  (* crtcls assumes that the code lies in register r_t1 and the variable lies in r_t2 *)
   Definition crtcls_instrs f_m :=
-    encodeInstrsLW [Mov r_t6 r_t1; Mov r_t7 r_t2] ++
-    malloc_instrs f_m 8%nat ++
-    scrtcls_instrs r_t6 r_t7.
+    encodeInstrsLW [ Mov r_t6 r_t1
+                  ; Mov r_t7 r_t2
+                  ] ++ malloc_instrs f_m 8%nat
+                  ++ scrtcls_instrs r_t6 r_t7.
 
-  Definition crtcls f_m a v : iProp Σ :=
-    ([∗ list] a_i;w_i ∈ a;(crtcls_instrs f_m), (a_i, v) ↦ₐ w_i)%I.
+  Lemma scrtcls_spec rcode rdata wvar wcode pc_p pc_b pc_e v a_first act_b act_e act φ :
+    ExecPCPerm pc_p →
+    SubBounds pc_b pc_e a_first (a_first ^+ length (scrtcls_instrs rcode rdata))%a →
 
-  (* scrtcls *)
-  Lemma scrtcls_spec rcode rdata wvar wcode a pc_p pc_b pc_e v a_first a_last
-        act_b act_e act φ :
-    isCorrectPC_range pc_p pc_b pc_e a_first a_last →
-    contiguous_between a a_first a_last →
     (act_b + 8)%a = Some act_e →
 
-      ▷ scrtcls rcode rdata a v
+    ▷ codefrag a_first v (scrtcls_instrs rcode rdata)
     ∗ ▷ PC ↦ᵣ LCap pc_p pc_b pc_e a_first v
     (* register state *)
     ∗ ▷ r_t1 ↦ᵣ LCap RWX act_b act_e act_b v
@@ -1565,7 +885,8 @@ Section macros.
     (* memory for the activation record *)
     ∗ ▷ ([[act_b,act_e]] ↦ₐ{v} [[ act ]])
     (* continuation *)
-    ∗ ▷ (PC ↦ᵣ LCap pc_p pc_b pc_e a_last v ∗ scrtcls rcode rdata a v
+    ∗ ▷ (PC ↦ᵣ LCap pc_p pc_b pc_e (a_first ^+ length (scrtcls_instrs rcode rdata))%a v
+         ∗ codefrag a_first v (scrtcls_instrs rcode rdata)
          ∗ r_t1 ↦ᵣ LCap E act_b act_e act_b v
          ∗ [[act_b,act_e]] ↦ₐ{v} [[ activation_instrs wcode wvar ]]
          ∗ rcode ↦ᵣ LInt 0%Z
@@ -1575,7 +896,9 @@ Section macros.
       WP Seq (Instr Executable) {{ φ }}.
   Proof.
     iIntros (Hvpc Hcont Hact) "(>Hprog & >HPC & >Hr_t1 & >Hrcode & >Hrdata & >Hact & Hφ)".
-    iDestruct (big_sepL2_length with "Hprog") as %Hlength.
+
+    (* TODO: This part is needed to have a concrete list, but could be automated as in codefrag_lookup_acc
+       to avoid this *)
     assert (act_b < act_e)%a as Hlt;[solve_addr|].
     opose proof (contiguous_between_region_addrs act_b act_e _) as Hcont_act; first solve_addr.
     unfold region_mapsto.
@@ -1584,189 +907,166 @@ Section macros.
     { rewrite Heqacta finz_seq_between_length. by apply finz_incr_iff_dist. }
     iDestruct (big_sepL2_length with "Hact") as %Hact_len.
     rewrite map_length Hact_len_a in Hact_len. symmetry in Hact_len.
-    repeat (destruct act as [| ? act]; try by inversion Hact_len).
-    clear Hact_len.
-    rename l into w.
-    destruct a as [|a l]; [inversion Hlength|].
-    apply contiguous_between_cons_inv_first in Hcont as Heq. subst a.
+    repeat (destruct act as [| ? act]; try by inversion Hact_len). clear Hact_len.
     assert (∀ i a', acta !! i = Some a' → withinBounds act_b act_e a' = true) as Hwbact.
     { intros i a' Hsome. apply andb_true_intro. subst acta.
       apply contiguous_between_incr_addr with (i:=i) (ai:=a') in Hcont_act. 2: done.
-      apply lookup_lt_Some in Hsome. split;[apply Z.leb_le|apply Z.ltb_lt]; solve_addr.
-    }
-    (* store_z r_t1 v1 *)
-    destruct l; [inversion Hlength|].
-    destruct acta as [| a0 acta]; [inversion Hact_len_a|].
-    assert (a0 = act_b) as ->.
-    { opose proof (finz_seq_between_first act_b act_e _) as HH; first solve_addr.
-      rewrite -Heqacta /= in HH. by inversion HH. }
+      apply lookup_lt_Some in Hsome. split;[apply Z.leb_le|apply Z.ltb_lt]; solve_addr. }
+    repeat (destruct acta as [|? acta]; try by inversion Hact_len_a). clear Hact_len_a.
+    replace f with act_b in * by (symmetry; eapply contiguous_between_cons_inv_first; eauto).
+
+    iDestruct "Hact" as "[Hact_b Hact]".
     iDestruct "Hact" as "[Ha0 Hact]".
-    iPrologue "Hprog".
-    iApply (wp_store_success_z with "[$HPC $Hi $Ha0 $Hr_t1]");
-      [apply decode_encode_instrLW_inv|iCorrectLPC a_first a_last|iContiguous_next Hcont 0|..]; auto.
-    { apply Hwbact with 0. auto. }
-    iEpilogue "(HPC & Hi & Hr_t1 & Hact')"; iRename "Hi" into "Hprog_done".
-    (* lea r_t1 1 *)
-    destruct l;[inversion Hlength|].
-    destruct acta as [| a1 acta]; [inversion Hact_len_a|].
-    iPrologue "Hprog".
-    iApply (wp_lea_success_z with "[$HPC $Hi $Hr_t1]");
-      [apply decode_encode_instrLW_inv|iCorrectLPC a_first a_last|iContiguous_next Hcont 1|
-       iContiguous_next Hcont_act 0|simpl;auto..].
-    iEpilogue "(HPC & Hi & Hr_t1)"; iCombine "Hi" "Hprog_done" as "Hprog_done".
-    (* store_z r_t1 v2 *)
-    destruct l;[inversion Hlength|].
-    iPrologue "Hprog".
     iDestruct "Hact" as "[Ha1 Hact]".
-    iApply (wp_store_success_z with "[$HPC $Hi $Hr_t1 $Ha1]");
-      [apply decode_encode_instrLW_inv|iCorrectLPC a_first a_last|iContiguous_next Hcont 2|..]; auto.
-    { apply Hwbact with 1. auto. }
-    iEpilogue "(HPC & Hi & Hr_t1 & Ha1)"; iCombine "Hi" "Hprog_done" as "Hprog_done"; iCombine "Ha1" "Hact'" as "Hact'".
-    (* lea r_t1 1 *)
-    destruct l;[inversion Hlength|].
-    destruct acta as [| ? acta];[inversion Hact_len_a|].
-    iPrologue "Hprog".
-    iApply (wp_lea_success_z with "[$HPC $Hi $Hr_t1]");
-      [apply decode_encode_instrLW_inv|iCorrectLPC a_first a_last|iContiguous_next Hcont 3|
-       iContiguous_next Hcont_act 1|simpl;auto..].
-    iEpilogue "(HPC & Hi & Hr_t1)"; iCombine "Hi" "Hprog_done" as "Hprog_done".
-    (* store_z r_t1 v3 *)
-    destruct l;[inversion Hlength|].
-    iPrologue "Hprog".
     iDestruct "Hact" as "[Ha2 Hact]".
-    iApply (wp_store_success_z with "[$HPC $Hi $Hr_t1 $Ha2]");
-      [apply decode_encode_instrLW_inv|iCorrectLPC a_first a_last|iContiguous_next Hcont 4|..]; auto.
-    { apply Hwbact with 2. auto. }
-    iEpilogue "(HPC & Hi & Hr_t1 & Ha2)"; iCombine "Hi" "Hprog_done" as "Hprog_done"; iCombine "Ha2" "Hact'" as "Hact'".
-    (* lea r_t1 1 *)
-    destruct l;[inversion Hlength|].
-    destruct acta as [| ? acta];[inversion Hact_len_a|].
-    iPrologue "Hprog".
-    iApply (wp_lea_success_z with "[$HPC $Hi $Hr_t1]");
-      [apply decode_encode_instrLW_inv|iCorrectLPC a_first a_last|iContiguous_next Hcont 5|
-       iContiguous_next Hcont_act 2|simpl;auto..].
-    iEpilogue "(HPC & Hi & Hr_t1)"; iCombine "Hi" "Hprog_done" as "Hprog_done".
-    (* store_z r_t1 v4 *)
-    destruct l;[inversion Hlength|].
-    iPrologue "Hprog".
     iDestruct "Hact" as "[Ha3 Hact]".
-    iApply (wp_store_success_z with "[$HPC $Hi $Hr_t1 $Ha3]");
-      [apply decode_encode_instrLW_inv|iCorrectLPC a_first a_last|iContiguous_next Hcont 6|..]; auto.
-    { apply Hwbact with 3. auto. }
-    iEpilogue "(HPC & Hi & Hr_t1 & Ha3)"; iCombine "Hi" "Hprog_done" as "Hprog_done"; iCombine "Ha3" "Hact'" as "Hact'".
-    (* lea r_t1 1 *)
-    destruct l;[inversion Hlength|].
-    destruct acta as [| ? acta];[inversion Hact_len_a|].
-    iPrologue "Hprog".
-    iApply (wp_lea_success_z with "[$HPC $Hi $Hr_t1]");
-      [apply decode_encode_instrLW_inv|iCorrectLPC a_first a_last|iContiguous_next Hcont 7|
-       iContiguous_next Hcont_act 3|simpl;auto..].
-    iEpilogue "(HPC & Hi & Hr_t1)"; iCombine "Hi" "Hprog_done" as "Hprog_done".
-    (* store_z r_t1 v5 *)
-    destruct l;[inversion Hlength|].
-    iPrologue "Hprog".
     iDestruct "Hact" as "[Ha4 Hact]".
-    iApply (wp_store_success_z with "[$HPC $Hi $Hr_t1 $Ha4]");
-      [apply decode_encode_instrLW_inv|iCorrectLPC a_first a_last|iContiguous_next Hcont 8|..]; auto.
-    { apply Hwbact with 4. auto. }
-    iEpilogue "(HPC & Hi & Hr_t1 & Ha4)"; iCombine "Hi" "Hprog_done" as "Hprog_done"; iCombine "Ha4" "Hact'" as "Hact'".
-    (* lea r_t1 1 *)
-    destruct l;[inversion Hlength|].
-    destruct acta as [| ? acta];[inversion Hact_len_a|].
-    iPrologue "Hprog".
-    iApply (wp_lea_success_z with "[$HPC $Hi $Hr_t1]");
-      [apply decode_encode_instrLW_inv|iCorrectLPC a_first a_last|iContiguous_next Hcont 9|
-       iContiguous_next Hcont_act 4|simpl;auto..].
-    iEpilogue "(HPC & Hi & Hr_t1)"; iCombine "Hi" "Hprog_done" as "Hprog_done".
-    (* store_z r_t1 v6 *)
-    destruct l;[inversion Hlength|].
-    iPrologue "Hprog".
     iDestruct "Hact" as "[Ha5 Hact]".
-    iApply (wp_store_success_z with "[$HPC $Hi $Hr_t1 $Ha5]");
-      [apply decode_encode_instrLW_inv|iCorrectLPC a_first a_last|iContiguous_next Hcont 10|..]; auto.
-    { apply Hwbact with 5. auto. }
-    iEpilogue "(HPC & Hi & Hr_t1 & Ha5)"; iCombine "Hi" "Hprog_done" as "Hprog_done"; iCombine "Ha5" "Hact'" as "Hact'".
-    (* lea r_t1 1 *)
-    destruct l;[inversion Hlength|].
-    destruct acta as [| ? acta];[inversion Hact_len_a|].
-    iPrologue "Hprog".
-    iApply (wp_lea_success_z with "[$HPC $Hi $Hr_t1]");
-      [apply decode_encode_instrLW_inv|iCorrectLPC a_first a_last|iContiguous_next Hcont 11|
-       iContiguous_next Hcont_act 5|simpl;auto..].
-    iEpilogue "(HPC & Hi & Hr_t1)"; iCombine "Hi" "Hprog_done" as "Hprog_done".
-    (* store r_t1 rcode *)
-    destruct l;[inversion Hlength|].
-    iPrologue "Hprog".
     iDestruct "Hact" as "[Ha6 Hact]".
-    iApply (wp_store_success_reg with "[$HPC $Hi $Ha6 $Hrcode $Hr_t1]");
-      [apply decode_encode_instrLW_inv|iCorrectLPC a_first a_last|iContiguous_next Hcont 12|..]; auto.
-    { apply Hwbact with 6. auto. }
-    iEpilogue "(HPC & Hi & Hrcode & Hr_t1 & Ha6)"; iCombine "Hi" "Hprog_done" as "Hprog_done"; iCombine "Ha6" "Hact'" as "Hact'".
-    (* move rcode 0 *)
-    destruct l;[inversion Hlength|].
-    iPrologue "Hprog".
-    iApply (wp_move_success_z with "[$HPC $Hi $Hrcode]");
-      [apply decode_encode_instrLW_inv|iCorrectLPC a_first a_last|iContiguous_next Hcont 13|auto..].
-    iEpilogue "(HPC & Hi & Hrcode)"; iCombine "Hi" "Hprog_done" as "Hprog_done".
-    (* lea r_t1 1 *)
-    destruct l;[inversion Hlength|].
-    destruct acta as [| ? acta];[inversion Hact_len_a|].
-    iPrologue "Hprog".
-    iApply (wp_lea_success_z with "[$HPC $Hi $Hr_t1]");
-      [apply decode_encode_instrLW_inv|iCorrectLPC a_first a_last|iContiguous_next Hcont 14|
-       iContiguous_next Hcont_act 6|simpl;auto..].
-    iEpilogue "(HPC & Hi & Hr_t1)"; iCombine "Hi" "Hprog_done" as "Hprog_done".
-    (* store r_t1 rdata *)
-    destruct l;[inversion Hlength|].
-    iPrologue "Hprog".
-    iDestruct "Hact" as "[Ha7 Hact]".
-    iApply (wp_store_success_reg with "[$HPC $Hi $Ha7 $Hrdata $Hr_t1]");
-      [apply decode_encode_instrLW_inv|iCorrectLPC a_first a_last|iContiguous_next Hcont 15|..]; auto.
-    { apply Hwbact with 7. auto. }
-    iEpilogue "(HPC & Hi & Hrdata & Hr_t1 & Ha7)"; iCombine "Hi" "Hprog_done" as "Hprog_done"; iCombine "Ha7" "Hact'" as "Hact'".
-    (* move rdata 0 *)
-    destruct l;[inversion Hlength|].
-    iPrologue "Hprog".
-    iApply (wp_move_success_z with "[$HPC $Hi $Hrdata]");
-      [apply decode_encode_instrLW_inv|iCorrectLPC a_first a_last|iContiguous_next Hcont 16|auto..].
-    iEpilogue "(HPC & Hi & Hrdata)"; iCombine "Hi" "Hprog_done" as "Hprog_done".
-    (* lea r_t1 -7 *)
-    destruct l;[by inversion Hlength|].
-    destruct acta as [| ? acta];[| by inversion Hact_len_a].
-    iPrologue "Hprog".
-    apply contiguous_between_last with (ai:=f19) in Hcont_act as Hnext; auto.
-    assert ((f19 + (-7))%a = Some act_b) as Hlea.
-    { apply contiguous_between_length in Hcont_act. revert Hnext Hact; clear. solve_addr. }
-    iApply (wp_lea_success_z with "[$HPC $Hi $Hr_t1]");
-      [apply decode_encode_instrLW_inv|iCorrectLPC a_first a_last|iContiguous_next Hcont 17|apply Hlea|simpl;auto..].
-    iEpilogue "(HPC & Hi & Hr_t1)";iCombine "Hi" "Hprog_done" as "Hprog_done".
-    (* restrict r_t1 (Global,E) *)
-    destruct l;[|by inversion Hlength].
-    apply contiguous_between_last with (ai:=f22) in Hcont as Hlast; auto.
-    iPrologue "Hprog". iClear "Hprog".
-    iApply (wp_restrict_success_z with "[$HPC $Hi $Hr_t1]");
-      [apply decode_encode_instrLW_inv|iCorrectLPC a_first a_last|apply Hlast|auto..].
-    { rewrite decode_encode_perm_inv. auto. }
-    rewrite decode_encode_perm_inv.
-    iEpilogue "(HPC & Hi & Hr_t1)"; iCombine "Hi" "Hprog_done" as "Hprog_done".
-    (* continuation *)
-    iApply "Hφ".
-    iFrame "HPC". iSplitL "Hprog_done".
-    { do 21 iDestruct "Hprog_done" as "[$ Hprog_done]". iFrame. done. }
-    iFrame. do 7 iDestruct "Hact'" as "[$ Hact']". iFrame.
+    destruct (contiguous_between_cons_inv _ _ _ _ Hcont_act) as [_ [? [? HA0] ] ].
+    destruct (contiguous_between_cons_inv _ _ _ _ HA0) as [<- [? [? HA1] ] ]; clear HA0.
+    destruct (contiguous_between_cons_inv _ _ _ _ HA1) as [<- [? [? HA0] ] ]; clear HA1.
+    destruct (contiguous_between_cons_inv _ _ _ _ HA0) as [<- [? [? HA1] ] ]; clear HA0.
+    destruct (contiguous_between_cons_inv _ _ _ _ HA1) as [<- [? [? HA0] ] ]; clear HA1.
+    destruct (contiguous_between_cons_inv _ _ _ _ HA0) as [<- [? [? HA1] ] ]; clear HA0.
+    destruct (contiguous_between_cons_inv _ _ _ _ HA1) as [<- [? [? HA0] ] ]; clear HA1.
+    destruct (contiguous_between_cons_inv _ _ _ _ HA0) as [<- [? [? HA1] ] ]; clear HA0 HA1 H6 x.
+    generalize (contiguous_between_last _ _ _ f6 Hcont_act ltac:(reflexivity)); intros.
+
+    codefrag_facts "Hprog".
+    iInstr "Hprog". eapply (Hwbact 0); reflexivity.
+    iInstr "Hprog".
+    iInstr "Hprog". eapply (Hwbact 1); reflexivity.
+    iInstr "Hprog".
+    iInstr "Hprog". eapply (Hwbact 2); reflexivity.
+    iInstr "Hprog".
+    iInstr "Hprog". eapply (Hwbact 3); reflexivity.
+    iInstr "Hprog".
+    iInstr "Hprog". eapply (Hwbact 4); reflexivity.
+    iInstr "Hprog".
+    iInstr "Hprog". eapply (Hwbact 5); reflexivity.
+    iInstr "Hprog".
+    iInstr "Hprog". eapply (Hwbact 6); reflexivity.
+    iGo "Hprog". eapply (Hwbact 7); reflexivity.
+    iGo "Hprog". instantiate (1:= act_b). solve_addr.
+    iInstr "Hprog". rewrite /e decode_encode_perm_inv //.
+    iApply "Hφ". iFrame. rewrite /e decode_encode_perm_inv //.
   Qed.
 
-  (* crtcls spec *)
-  Lemma crtcls_spec f_m wvar wcode a pc_p pc_b pc_e v
-        a_first a_last b_link a_link e_link a_entry b_m e_m mallocN EN rmap cont φ :
-    isCorrectPC_range pc_p pc_b pc_e a_first a_last →
-    contiguous_between a a_first a_last →
+  Lemma crtcls_spec_alt f_m wvar wcode pc_p pc_b pc_e v
+        a_first b_link a_link e_link a_entry b_m e_m mallocN EN rmap cont φ ψ:
+    ExecPCPerm pc_p →
+    SubBounds pc_b pc_e a_first (a_first ^+ length (crtcls_instrs f_m))%a →
+
     withinBounds b_link e_link a_entry = true →
     (a_link + f_m)%a = Some a_entry →
     dom rmap = all_registers_s ∖ {[ PC; r_t0; r_t1; r_t2 ]} →
     ↑mallocN ⊆ EN →
 
-      ▷ crtcls f_m a v
+    ▷ codefrag a_first v (crtcls_instrs f_m)
+    ∗ ▷ PC ↦ᵣ LCap pc_p pc_b pc_e a_first v
+    ∗ na_inv logrel_nais mallocN (malloc_inv b_m e_m v)
+    ∗ na_own logrel_nais EN
+    (* we need to assume that the malloc capability is in the linking table at offset 0 *)
+    ∗ ▷ (pc_b,v) ↦ₐ LCap RO b_link e_link a_link v
+    ∗ ▷ (a_entry,v) ↦ₐ LCap E b_m e_m b_m v
+    (* register state *)
+    ∗ ▷ r_t0 ↦ᵣ cont
+    ∗ ▷ r_t1 ↦ᵣ wcode
+    ∗ ▷ r_t2 ↦ᵣ wvar
+    ∗ ▷ ([∗ map] r_i↦w_i ∈ rmap, r_i ↦ᵣ w_i)
+    ∗ ▷ (∀ v, ψ v -∗ φ v)
+    ∗ ▷ (φ FailedV)
+    (* continuation *)
+    ∗ ▷ (PC ↦ᵣ LCap pc_p pc_b pc_e (a_first ^+ length (crtcls_instrs f_m))%a v
+         ∗ codefrag a_first v (crtcls_instrs f_m)
+         ∗ (pc_b,v) ↦ₐ LCap RO b_link e_link a_link v
+         ∗ (a_entry,v) ↦ₐ LCap E b_m e_m b_m v
+         (* the newly allocated region *)
+         ∗ (∃ (b e : Addr), ⌜(b + 8)%a = Some e⌝ ∧ r_t1 ↦ᵣ LCap E b e b v
+         ∗ [[b,e]] ↦ₐ{v} [[ activation_instrs wcode wvar ]]
+         ∗ r_t0 ↦ᵣ cont
+         ∗ r_t2 ↦ᵣ LInt 0%Z
+         ∗ na_own logrel_nais EN
+         ∗ ([∗ map] r_i↦w_i ∈ <[r_t3:=LInt 0%Z]>
+                               (<[r_t4:=LInt 0%Z]>
+                                (<[r_t5:=LInt 0%Z]>
+                                 (<[r_t6:=LInt 0%Z]>
+                                  (<[r_t7:=LInt 0%Z]> rmap)))), r_i ↦ᵣ w_i))
+         -∗ WP Seq (Instr Executable) {{ ψ }})
+    ⊢
+      WP Seq (Instr Executable) {{ λ v, φ v }}.
+  Proof.
+    iIntros (Hvpc Hcont Hwb Ha_entry Hrmap_dom HmallocN)
+            "(>Hprog & >HPC & #Hmalloc & Hna & >Hpc_b & >Ha_entry & >Hr_t0 & >Hr_t1 & >Hr_t2 & >Hregs & Hψ & Hφfailed & Hφ)".
+    (* extract necessary registers from regs *)
+    assert (is_Some (rmap !! r_t6)) as [rv6 ?]. by rewrite -elem_of_dom Hrmap_dom; set_solver.
+    iDestruct (big_sepM_delete _ _ r_t6 with "Hregs") as "[Hr_t6 Hregs]"; eauto.
+    assert (is_Some (rmap !! r_t7)) as [rv7 ?]. by rewrite -elem_of_dom Hrmap_dom; set_solver.
+    iDestruct (big_sepM_delete _ _ r_t7 with "Hregs") as "[Hr_t7 Hregs]". by rewrite lookup_delete_ne //.
+
+    focus_block_0 "Hprog" as "Hsetup" "Hcont".
+    iGo "Hsetup".
+    unfocus_block "Hsetup" "Hcont" as "Hprog".
+
+    iDestruct (big_sepM_insert _ _ r_t6 with "[$Hregs $Hr_t6]") as "Hregs".
+      by simplify_map_eq.
+    iDestruct (big_sepM_insert _ _ r_t7 with "[$Hregs $Hr_t7]") as "Hregs".
+      by simplify_map_eq.
+    iDestruct (big_sepM_insert _ _ r_t1 with "[$Hregs $Hr_t1]") as "Hregs".
+      simplify_map_eq. eapply not_elem_of_dom. set_solver.
+    iDestruct (big_sepM_insert _ _ r_t2 with "[$Hregs $Hr_t2]") as "Hregs".
+      simplify_map_eq. eapply not_elem_of_dom. set_solver.
+    map_simpl "Hregs".
+
+    focus_block 1 "Hprog" as amid1 Hamid1 "Hmallocprog" "Hcont".
+    iApply malloc_spec_alt; iFrameAutoSolve; eauto; try iFrame "∗ #".
+    { rewrite !dom_insert_L. rewrite Hrmap_dom.
+      repeat (rewrite singleton_union_difference_L all_registers_union_l).
+      f_equal. }
+    { lia. }
+    iNext. iIntros "(HPC & Hmallocprog & Hpc_b & Ha_entry & Hbe & Hr_t0 & Hna & Hregs)".
+    unfocus_block "Hmallocprog" "Hcont" as "Hprog".
+
+    iDestruct "Hbe" as (b e Hbe) "(Hr_t1 & Hbe)".
+    focus_block 2 "Hprog" as amid2 Hmid2 "Hscrtcls" "Hcont".
+    map_simpl "Hregs".
+
+    iDestruct (big_sepM_delete _ _ r_t6 with "Hregs") as "[Hr_t6 Hregs]"; eauto.
+      by simplify_map_eq.
+    iDestruct (big_sepM_delete _ _ r_t7 with "Hregs") as "[Hr_t7 Hregs]"; eauto.
+      by simplify_map_eq.
+    map_simpl "Hregs".
+
+    iApply scrtcls_spec; iFrameAutoSolve; iFrame "∗".
+    iNext. iIntros "(HPC & Hscrtcls & Hr_t1 & Hbe & Hr_t6 & Hr_t7)".
+    iDestruct (big_sepM_insert _ _ r_t6 with "[$Hregs $Hr_t6]") as "Hregs".
+      by simplify_map_eq.
+    iDestruct (big_sepM_insert _ _ r_t7 with "[$Hregs $Hr_t7]") as "Hregs".
+      by simplify_map_eq.
+    iDestruct (big_sepM_delete _ _ r_t2 with "Hregs") as "[Hr_t2 Hregs]"; eauto.
+      by simplify_map_eq.
+    map_simpl "Hregs".
+    unfocus_block "Hscrtcls" "Hcont" as "Hprog".
+    changePCto (a_first ^+ length (crtcls_instrs f_m))%a.
+    iApply "Hφ". iFrame "∗".
+    iExists _,_. iSplitR; [eauto|]. iFrame "∗".
+    rewrite (delete_notin); [ | apply not_elem_of_dom_1; clear -Hrmap_dom; set_solver].
+    rewrite (delete_notin); [ | apply not_elem_of_dom_1; clear -Hrmap_dom; set_solver].
+    clear -Hrmap_dom; iFrameMapSolve "Hregs".
+  Qed.
+
+  Lemma crtcls_spec f_m wvar wcode pc_p pc_b pc_e v
+        a_first b_link a_link e_link a_entry b_m e_m mallocN EN rmap cont φ :
+    ExecPCPerm pc_p →
+    SubBounds pc_b pc_e a_first (a_first ^+ length (crtcls_instrs f_m))%a →
+
+    withinBounds b_link e_link a_entry = true →
+    (a_link + f_m)%a = Some a_entry →
+    dom rmap = all_registers_s ∖ {[ PC; r_t0; r_t1; r_t2 ]} →
+    ↑mallocN ⊆ EN →
+
+    ▷ codefrag a_first v (crtcls_instrs f_m)
     ∗ ▷ PC ↦ᵣ LCap pc_p pc_b pc_e a_first v
     ∗ na_inv logrel_nais mallocN (malloc_inv b_m e_m v)
     ∗ na_own logrel_nais EN
@@ -1779,7 +1079,8 @@ Section macros.
     ∗ ▷ r_t2 ↦ᵣ wvar
     ∗ ▷ ([∗ map] r_i↦w_i ∈ rmap, r_i ↦ᵣ w_i)
     (* continuation *)
-    ∗ ▷ (PC ↦ᵣ LCap pc_p pc_b pc_e a_last v ∗ crtcls f_m a v
+    ∗ ▷ (PC ↦ᵣ LCap pc_p pc_b pc_e (a_first ^+ length (crtcls_instrs f_m))%a v
+         ∗ codefrag a_first v (crtcls_instrs f_m)
          ∗ (pc_b,v) ↦ₐ LCap RO b_link e_link a_link v
          ∗ (a_entry,v) ↦ₐ LCap E b_m e_m b_m v
          (* the newly allocated region *)
@@ -1799,188 +1100,64 @@ Section macros.
   Proof.
     iIntros (Hvpc Hcont Hwb Ha_entry Hrmap_dom HmallocN)
             "(>Hprog & >HPC & #Hmalloc & Hna & >Hpc_b & >Ha_entry & >Hr_t0 & >Hr_t1 & >Hr_t2 & >Hregs & Hφ)".
-    (* get some registers out of regs *)
-    iDestruct (big_sepL2_length with "Hprog") as %Hlength.
-    assert (is_Some (rmap !! r_t6)) as [rv6 ?]. by rewrite -elem_of_dom Hrmap_dom; set_solver.
-    iDestruct (big_sepM_delete _ _ r_t6 with "Hregs") as "[Hr_t6 Hregs]"; eauto.
-    assert (is_Some (rmap !! r_t7)) as [rv7 ?]. by rewrite -elem_of_dom Hrmap_dom; set_solver.
-    iDestruct (big_sepM_delete _ _ r_t7 with "Hregs") as "[Hr_t7 Hregs]". by rewrite lookup_delete_ne //.
-    destruct a as [|a l];[inversion Hlength|].
-    apply contiguous_between_cons_inv_first in Hcont as Heq. subst.
-    (* move r_t6 r_t1 *)
-    destruct l;[inversion Hlength|].
-    iPrologue "Hprog".
-    iApply (wp_move_success_reg with "[$HPC $Hi $Hr_t6 $Hr_t1]");
-      [apply decode_encode_instrLW_inv|iCorrectLPC a_first a_last|iContiguous_next Hcont 0|].
-    iEpilogue "(HPC & Hprog_done & Hr_t6 & Hr_t1)".
-    (* move r_t7 r_t2 *)
-    destruct l;[inversion Hlength|].
-    iPrologue "Hprog".
-    iApply (wp_move_success_reg with "[$HPC $Hi $Hr_t7 $Hr_t2]");
-      [apply decode_encode_instrLW_inv|iCorrectLPC a_first a_last|iContiguous_next Hcont 1|].
-    iEpilogue "(HPC & Hi & Hr_t7 & Hr_t2)"; iCombine "Hi Hprog_done" as "Hprog_done".
-    assert (contiguous_between (f0 :: l) f0 a_last) as Hcont'.
-    { apply contiguous_between_cons_inv in Hcont as [_ (? & ? & Hcont)].
-      apply contiguous_between_cons_inv in Hcont as [_ (? & ? & Hcont)].
-      pose proof (contiguous_between_cons_inv_first _ _ _ _ Hcont). subst. apply Hcont. }
-    (* malloc 8 *)
-    iDestruct ( (contiguous_betweenL_program_split _ _ (fun la w_i => la ↦ₐ w_i )%I) with "Hprog")
-        as (malloc_prog rest link) "(Hmalloc_prog & Hprog & #Hcont)";[apply Hcont'|].
-    iDestruct "Hcont" as %(Hcont_fetch & Hcont_rest & Heqapp & Hlink).
-    (* we start by putting the registers back together *)
-    iDestruct (big_sepM_insert with "[$Hregs $Hr_t6]") as "Hregs".
-      by rewrite lookup_delete_ne // lookup_delete.
-      rewrite delete_commute // insert_delete_insert.
-    iDestruct (big_sepM_insert with "[$Hregs $Hr_t7]") as "Hregs".
-      by rewrite lookup_insert_ne // lookup_delete.
-      rewrite (insert_commute _ r_t7 r_t6) // insert_delete_insert.
-    assert (∀ (r:RegName), r ∈ ({[PC;r_t0;r_t1;r_t2]} : gset RegName) → rmap !! r = None) as Hnotin_rmap.
-    { intros r Hr. eapply (@not_elem_of_dom _ _ (gset RegName)). typeclasses eauto.
-      rewrite Hrmap_dom. set_solver. }
-    iDestruct (big_sepM_insert with "[$Hregs $Hr_t2]") as "Hregs".
-      by rewrite !lookup_insert_ne //; apply Hnotin_rmap; set_solver.
-    iDestruct (big_sepM_insert with "[$Hregs $Hr_t1]") as "Hregs".
-      by rewrite !lookup_insert_ne //; apply Hnotin_rmap; set_solver.
-    (* apply the malloc spec *)
-    rewrite -/(malloc _ _ _).
-    iApply (malloc_spec with "[- $HPC $Hmalloc $Hna $Hpc_b $Ha_entry $Hr_t0 $Hregs $Hmalloc_prog]");
-      [|apply Hcont_fetch|apply Hwb|apply Ha_entry| |auto|lia|..].
-    { intros mid Hmid. apply isCorrectPC_inrange with a_first a_last; auto.
-      apply contiguous_between_bounds in Hcont_rest.
-      apply contiguous_between_incr_addr with (i:=2) (ai:=f0) in Hcont;auto.
-      revert Hcont Hcont_rest Hmid; clear. solve_addr. }
-    { rewrite !dom_insert_L. rewrite Hrmap_dom.
-      repeat (rewrite singleton_union_difference_L all_registers_union_l).
-      f_equal. }
-    iNext. iIntros "(HPC & Hmalloc_prog & Hpc_b & Ha_entry & Hbe & Hr_t0 & Hna & Hregs)".
-    iDestruct "Hbe" as (b e Hbe) "(Hr_t1 & Hbe)".
-    rewrite delete_insert_delete.
-    rewrite (delete_insert_ne _ r_t1 r_t2) //.
-    repeat (rewrite (insert_commute _ _ r_t2) //;[]).
-    rewrite insert_insert.
-    iDestruct (big_sepM_delete _ _ r_t6 with "Hregs") as "[Hr_t6 Hregs]".
-      by rewrite !lookup_insert_ne // lookup_delete_ne // lookup_insert //.
-    iDestruct (big_sepM_delete _ _ r_t7 with "Hregs") as "[Hr_t7 Hregs]".
-      rewrite lookup_delete_ne // !lookup_insert_ne // lookup_delete_ne //
-              lookup_insert_ne // lookup_insert //.
-    iApply (scrtcls_spec with "[- $Hprog $HPC $Hr_t1 $Hr_t6 $Hr_t7 $Hbe]"); eauto.
-    { intros mid Hmid. apply isCorrectPC_inrange with a_first a_last; auto.
-      apply contiguous_between_bounds in Hcont_rest.
-      apply contiguous_between_bounds in Hcont_fetch.
-      apply contiguous_between_incr_addr with (i:=2) (ai:=f0) in Hcont; auto.
-      revert Hmid Hcont_rest Hcont_fetch Hcont ; clear. solve_addr. }
-    iNext. iIntros "(HPC & Hscrtcls_prog & Hr_t1 & Hact & Hr_t6 & Hr_t7)".
-    (* continuation *)
-    iApply "Hφ". iFrame "HPC Hpc_b Ha_entry". iSplitL "Hprog_done Hmalloc_prog Hscrtcls_prog".
-    { rewrite Heqapp. iDestruct "Hprog_done" as "[? ?]". iFrame. }
-    iExists b,e. iSplitR;auto. iFrame.
-    iDestruct (big_sepM_delete _ _ r_t2 with "Hregs") as "[Hr_t2 Hregs]".
-      by do 2 (rewrite lookup_delete_ne //); rewrite lookup_insert //.
-    iFrame "Hr_t2".
-    iDestruct (big_sepM_insert with "[$Hregs $Hr_t6]") as "Hregs".
-      by do 2 (rewrite lookup_delete_ne //); rewrite lookup_delete //.
-    iDestruct (big_sepM_insert with "[$Hregs $Hr_t7]") as "Hregs".
-      by rewrite lookup_insert_ne // lookup_delete_ne // lookup_delete //.
-    repeat (repeat (rewrite delete_insert_ne //; []); rewrite delete_insert_delete).
-    rewrite (delete_notin _ r_t1). 2: apply Hnotin_rmap; set_solver.
-    rewrite (delete_notin _ r_t2). 2: rewrite !lookup_delete_ne //; apply Hnotin_rmap; set_solver.
-    repeat (rewrite -delete_insert_ne //; []). rewrite insert_delete_insert.
-    repeat (rewrite -delete_insert_ne //; []). rewrite insert_delete_insert.
-    repeat (rewrite (insert_commute _ r_t7) //;[]).
-    repeat (rewrite (insert_commute _ r_t6) //;[]). rewrite (insert_commute _ r_t6 r_t5) //.
+    iApply crtcls_spec_alt; iFrameAutoSolve; eauto. iFrame. iFrame "Hmalloc".
+    iSplitL. iNext. eauto. eauto.
   Qed.
 
   (* ------------------------------- Closure Activation --------------------------------- *)
 
   Lemma closure_activation_spec pc_p b_cls e_cls v r1v renvv wcode wenv φ :
-    readAllowed pc_p = true →
-    isCorrectPC_range pc_p b_cls e_cls b_cls e_cls →
-    pc_p ≠ E →
+    ExecPCPerm pc_p →
+
     PC ↦ᵣ LCap pc_p b_cls e_cls b_cls v
-    ∗ r_t1 ↦ᵣ r1v
+    ∗ r_t20 ↦ᵣ r1v
     ∗ r_env ↦ᵣ renvv
     ∗ [[b_cls, e_cls]] ↦ₐ{v} [[ activation_instrs wcode wenv ]]
-    ∗ (  PC ↦ᵣ updatePcPermL wcode
-       ∗ r_t1 ↦ᵣ wcode
+    ∗ ▷ (  PC ↦ᵣ updatePcPermL wcode
+       ∗ r_t20 ↦ᵣ wcode
        ∗ r_env ↦ᵣ wenv
        ∗ [[b_cls, e_cls]] ↦ₐ{v} [[ activation_instrs wcode wenv ]]
        -∗ WP Seq (Instr Executable) {{ φ }})
     ⊢
       WP Seq (Instr Executable) {{ φ }}.
   Proof.
-    iIntros (Hrpc Hvpc HnpcE) "(HPC & Hr1 & Hrenv & Hcls & Hcont)".
+    iIntros (Hrpc) "(HPC & Hr1 & Hrenv & Hprog & Hcont)".
     rewrite /region_mapsto.
-    iDestruct (big_sepL2_length with "Hcls") as %Hcls_len. simpl in Hcls_len.
+    iDestruct (big_sepL2_length with "Hprog") as %Hcls_len. simpl in Hcls_len.
     assert (b_cls + 8 = Some e_cls)%a as Hbe.
     { rewrite map_length finz_seq_between_length /finz.dist in Hcls_len.
       revert Hcls_len; clear; solve_addr. }
-    assert (contiguous_between (finz.seq_between b_cls e_cls) b_cls e_cls) as Hcont_cls.
-    { apply contiguous_between_of_region_addrs; auto. revert Hbe; clear; solve_addr. }
-    pose proof (finz_seq_between_NoDup b_cls e_cls) as Hcls_nodup.
-    iDestruct (big_sepL2_split_at 6 with "Hcls") as "[Hcls_code Hcls_data]".
-    cbn [take drop].
-    destruct (finz.seq_between b_cls e_cls) as [| ? ll]; [by inversion Hcls_len|].
-    pose proof (contiguous_between_cons_inv_first _ _ _ _ Hcont_cls). subst.
-    do 7 (destruct ll as [| ? ll]; [by inversion Hcls_len|]).
-    destruct ll;[| by inversion Hcls_len]. cbn [take drop].
-    iDestruct "Hcls_data" as "(Hcls_ptr & Hcls_env & _)".
-    (* move r_t1 PC *)
-    iPrologue "Hcls_code".
-    iApply (wp_move_success_reg_fromPC with "[$HPC $Hi $Hr1]");
-      [apply decode_encode_instrLW_inv| iCorrectLPC b_cls e_cls |
-       iContiguous_next Hcont_cls 0 |..].
-    iEpilogue "(HPC & Hprog_done & Hr1)".
-    (* lea r_t1 7 *)
-    iPrologue "Hprog".
-    iApply (wp_lea_success_z with "[$HPC $Hi $Hr1]");
-      [apply decode_encode_instrLW_inv | iCorrectLPC b_cls e_cls |
-       iContiguous_next Hcont_cls 1 | | done | ..].
-    { eapply contiguous_between_incr_addr_middle' with (i:=0); eauto.
-      cbn. clear. lia. }
-    iEpilogue "(HPC & Hi & Hr1)". iCombine "Hi Hprog_done" as "Hprog_done".
-    (* load r_env r_t1 *)
-    iPrologue "Hprog".
-    (* FIXME: tedious & fragile *)
-    assert ((f5 =? f0)%a = false) as H_5_0.
-    { apply Z.eqb_neq. intros Heqb. assert (f5 = f0) as ->. revert Heqb; clear; solve_addr.
-      exfalso. by pose proof (NoDup_lookup _ 2 7 _ Hcls_nodup eq_refl eq_refl). }
-    iApply (wp_load_success with "[$HPC $Hi $Hrenv $Hr1 Hcls_env]");
-      [apply decode_encode_instrLW_inv | iCorrectLPC b_cls e_cls |
-       split;[done|] | iContiguous_next Hcont_cls 2 | ..].
-    { eapply contiguous_between_middle_bounds' in Hcont_cls as [? ?].
-      by eapply le_addr_withinBounds; eauto. repeat constructor. }
-    { rewrite H_5_0. iFrame. }
-    iEpilogue "(HPC & Hrenv & Hi & Hr1 & Hcls_env)". rewrite H_5_0.
-    iCombine "Hi Hprog_done" as "Hprog_done".
-    (* lea r_t1 (-1) *)
-    iPrologue "Hprog".
-    iApply (wp_lea_success_z with "[$HPC $Hi $Hr1]");
-      [apply decode_encode_instrLW_inv | iCorrectLPC b_cls e_cls |
-       iContiguous_next Hcont_cls 3 | | done | ..].
-    { assert ((f4 + 1)%a = Some f5) as HH. by iContiguous_next Hcont_cls 6.
-      instantiate (1 := f4). revert HH. clear; solve_addr. }
-    iEpilogue "(HPC & Hi & Hr1)". iCombine "Hi Hprog_done" as "Hprog_done".
-    (* load r_t1 r_t1 *)
-    iPrologue "Hprog".
-    (* FIXME: tedious & fragile *)
-    assert ((f4 =? f2)%a = false) as H_4_2.
-    { apply Z.eqb_neq. intros Heqb. assert (f4 = f2) as ->. revert Heqb; clear; solve_addr.
-      exfalso. by pose proof (NoDup_lookup _ 4 6 _ Hcls_nodup eq_refl eq_refl). }
-    iApply (wp_load_success_same with "[$HPC $Hi $Hr1 Hcls_ptr]");
-      [(* FIXME *) auto | apply decode_encode_instrLW_inv | iCorrectLPC b_cls e_cls |
-       done | auto | iContiguous_next Hcont_cls 4 | ..].
-    { eapply contiguous_between_middle_bounds' in Hcont_cls as [? ?].
-      by eapply le_addr_withinBounds; eauto. repeat constructor. }
-    { rewrite H_4_2. iFrame. }
-    iEpilogue "(HPC & Hr1 & Hi & Hcls_ptr)". rewrite H_4_2.
-    iCombine "Hi Hprog_done" as "Hprog_done".
-    (* jmp r_t1 *)
-    iPrologue "Hprog".
-    iApply (wp_jmp_success with "[$HPC $Hi $Hr1]");
-      [apply decode_encode_instrLW_inv | iCorrectLPC b_cls e_cls | .. ].
-    iEpilogue "(HPC & Hi & Hr1)".
+    assert (∃ b_end, b_cls + 6 = Some b_end)%a as [b_end Hbend];[destruct (b_cls + 6)%a eqn:HH;eauto;exfalso;solve_addr|].
+    assert (∃ b_mid, b_cls + 7 = Some b_mid)%a as [b_mid Hbmid];[destruct (b_cls + 7)%a eqn:HH;eauto;exfalso;solve_addr|].
 
-    iApply "Hcont". do 4 (iDestruct "Hprog_done" as "(? & Hprog_done)"). iFrame.
+    iAssert (codefrag b_cls v (activation_code) ∗ (b_end,v) ↦ₐ wcode ∗ (b_mid,v) ↦ₐ wenv)%I with "[Hprog]" as "[Hprog [Henv Henv']]".
+    { rewrite /codefrag (_: b_cls ^+ length activation_code = b_end)%a /=; [|solve_addr].
+      rewrite /activation_instrs.
+      rewrite (finz_seq_between_split _ b_end);[|solve_addr].
+      rewrite map_app.
+      iDestruct (big_sepL2_app_inv with "Hprog") as "[Hprog Henv]". simpl.
+      rewrite map_length finz_seq_between_length /finz.dist. left. solve_addr.
+      iFrame. rewrite finz_seq_between_cons;[|solve_addr]. assert (b_end + 1 = Some b_mid)%a as ->%addr_incr_eq. solve_addr. simpl.
+      rewrite finz_seq_between_cons;[|solve_addr]. assert (b_mid + 1 = Some e_cls)%a as ->%addr_incr_eq. solve_addr. simpl.
+      iDestruct "Henv" as "($&$&_)". }
+
+    assert (readAllowed pc_p = true ∧ withinBounds b_cls e_cls b_mid = true) as [Hra Hwb].
+    { split;[|solve_addr]. inversion Hrpc;subst;auto. }
+    assert ((b_mid + -1)%a = Some b_end);[solve_addr|].
+    assert (withinBounds b_cls e_cls b_end = true) as Hwb';[solve_addr|].
+
+    assert (SubBounds b_cls e_cls b_cls (b_cls ^+ length (activation_code))%a). solve_addr.
+    codefrag_facts "Hprog".
+    iGo "Hprog". auto.
+    iGo "Hprog".
+    iApply "Hcont". iFrame.
+    rewrite /codefrag (_: b_cls ^+ length activation_code = b_end)%a; [| solve_addr]. rewrite /activation_instrs.
+    rewrite (finz_seq_between_split _ b_end);[|solve_addr].
+      rewrite map_app.
+    iApply (big_sepL2_app with "Hprog").
+    rewrite finz_seq_between_cons;[|solve_addr]. assert (b_end + 1 = Some b_mid)%a as ->%addr_incr_eq. solve_addr. simpl.
+    rewrite finz_seq_between_cons;[|solve_addr]. assert (b_mid + 1 = Some e_cls)%a as ->%addr_incr_eq. solve_addr. simpl.
+    iFrame. rewrite finz_seq_between_empty;[|solve_addr]. done.
   Qed.
 
 End macros.
