theories/examples/enclaves/trusted_compute_adequacy.v
@@ -1,7 +1,7 @@
 From iris.proofmode Require Import proofmode.
 From cap_machine Require Import rules logrel fundamental.
 From cap_machine Require Import proofmode.
-From cap_machine Require Import assert macros_new.
+From cap_machine Require Import assert macros.
 From cap_machine Require Import template_adequacy_attestation.
 From cap_machine Require Import
   trusted_compute_code
